Add missing files and ensure IsaBIL.thy builds

Parser/Parser.thy
@@ -5,10 +5,12 @@ begin
 
 
 fun
-  parse_nat :: \<open>AST \<Rightarrow> nat parser_result\<close>
+  parse_nat_radix :: \<open>nat \<Rightarrow> AST \<Rightarrow> nat parser_result\<close>
 where
-  \<open>parse_nat (Node str []) = map_result_error (List.append (List.append ''Failed to parse string as nat: '' str)) (nat_of_string str)\<close> |
-  \<open>parse_nat (Node str (x # xs)) = Error (List.append (List.append ''Expecting no arguments for type "nat" ('' str) ''), got many.'')\<close>
+  \<open>parse_nat_radix radix (Node str []) = map_result_error (List.append (List.append ''Failed to parse string as nat: '' str)) (nat_of_string_radix radix str)\<close> |
+  \<open>parse_nat_radix radix (Node str (x # xs)) = Error (List.append (List.append ''Expecting no arguments for type "nat" ('' str) ''), got many.'')\<close>
+
+abbreviation \<open>parse_nat_dec \<equiv> parse_nat_radix 10\<close>
 
 fun
   parse_int :: \<open>AST \<Rightarrow> int parser_result\<close>
@@ -44,8 +46,8 @@ termination by lexicographic_order
 function
   parse_typ :: \<open>AST \<Rightarrow> Type parser_result\<close>
 where
-  \<open>parse_typ (Node ''Imm'' [sz]) = map_result_value Imm (parse_nat sz)\<close> |
-  \<open>parse_typ (Node ''Mem'' [sz\<^sub>a\<^sub>d\<^sub>d\<^sub>r, sz\<^sub>m\<^sub>e\<^sub>m]) = map_result_value2 Mem (parse_nat sz\<^sub>a\<^sub>d\<^sub>d\<^sub>r) (parse_nat sz\<^sub>m\<^sub>e\<^sub>m)\<close> |
+  \<open>parse_typ (Node ''Imm'' [sz]) = map_result_value Imm (parse_nat_dec sz)\<close> |
+  \<open>parse_typ (Node ''Mem'' [sz\<^sub>a\<^sub>d\<^sub>d\<^sub>r, sz\<^sub>m\<^sub>e\<^sub>m]) = map_result_value2 Mem (parse_nat_dec sz\<^sub>a\<^sub>d\<^sub>d\<^sub>r) (parse_nat_dec sz\<^sub>m\<^sub>e\<^sub>m)\<close> |
   \<open>\<lbrakk>length asts \<noteq> 1\<rbrakk> \<Longrightarrow> parse_typ (Node ''Imm'' asts) = Error ''Expecting 1 argument for type "Imm", got many.''\<close> |
   \<open>\<lbrakk>length asts \<noteq> 2\<rbrakk> \<Longrightarrow> parse_typ (Node ''Mem'' asts) = Error ''Expecting 2 arguments for type "Mem", got many.''\<close> |
   \<open>\<lbrakk>typ \<noteq> ''Imm''; typ \<noteq> ''Mem''\<rbrakk> \<Longrightarrow> parse_typ (Node typ _) = Error (List.append ''Expecting either Imm or Mem but received: '' typ)\<close>
@@ -77,10 +79,10 @@ termination by lexicographic_order
 function
   parse_exp :: \<open>AST \<Rightarrow> exp parser_result\<close>
 where
-  \<open>parse_exp (Node ''Store'' [e\<^sub>1, e\<^sub>2, e\<^sub>3, en, sz]) = map_result_value5 Store (parse_exp e\<^sub>1) (parse_exp e\<^sub>2) (parse_en en) (parse_nat sz) (parse_exp e\<^sub>3)\<close> |
+  \<open>parse_exp (Node ''Store'' [e\<^sub>1, e\<^sub>2, e\<^sub>3, en, sz]) = map_result_value5 Store (parse_exp e\<^sub>1) (parse_exp e\<^sub>2) (parse_en en) (parse_nat_dec sz) (parse_exp e\<^sub>3)\<close> |
   \<open>\<lbrakk>length ast \<noteq> 5\<rbrakk> \<Longrightarrow> parse_exp (Node ''Store'' ast) = Error ''Expecting 5 arguments for type "Store", got many.''\<close> |
 
-  \<open>parse_exp (Node ''Load'' [e\<^sub>1, e\<^sub>2, en, sz]) = map_result_value4 Load (parse_exp e\<^sub>1) (parse_exp e\<^sub>2) (parse_en en) (parse_nat sz)\<close> |
+  \<open>parse_exp (Node ''Load'' [e\<^sub>1, e\<^sub>2, en, sz]) = map_result_value4 Load (parse_exp e\<^sub>1) (parse_exp e\<^sub>2) (parse_en en) (parse_nat_dec sz)\<close> |
   \<open>\<lbrakk>length ast \<noteq> 4\<rbrakk> \<Longrightarrow> parse_exp (Node ''Load'' ast) = Error ''Expecting 4 arguments for type "Load", got many.''\<close> |
 
   \<open>parse_exp (Node ''Var'' asts) = map_result_value EVar (parse_var (Node ''Var'' asts))\<close> |
@@ -88,7 +90,7 @@ where
   \<open>parse_exp (Node ''Let'' [var, e\<^sub>1, e\<^sub>2]) = map_result_value3 Let (parse_var var) (parse_exp e\<^sub>1) (parse_exp e\<^sub>2)\<close> |
   \<open>\<lbrakk>length ast \<noteq> 3\<rbrakk> \<Longrightarrow> parse_exp (Node ''Let'' ast) = Error ''Expecting 3 arguments for type "Let", got many.''\<close> |
 
-  \<open>parse_exp (Node ''Int'' [num, sz]) = map_result_value Val (map_result_value Immediate (map_result_value2 Word (parse_nat num) (parse_nat sz)))\<close> |
+  \<open>parse_exp (Node ''Int'' [num, sz]) = map_result_value Val (map_result_value Immediate (map_result_value2 Word (parse_nat_dec num) (parse_nat_dec sz)))\<close> |
   \<open>\<lbrakk>length ast \<noteq> 2\<rbrakk> \<Longrightarrow> parse_exp (Node ''Int'' ast) = Error ''Expecting 2 arguments for type "Int", got many.''\<close> |
 
   \<open>parse_exp (Node ''Unknown'' [str, t]) = map_result_value Val (map_result_value2 Unknown (parse_str str) (parse_typ t))\<close> |
@@ -148,16 +150,16 @@ where
   \<open>parse_exp (Node ''LSHIFT'' [e\<^sub>1, e\<^sub>2]) = map_result_value2 (\<lambda>e\<^sub>1 e\<^sub>2. BinOp e\<^sub>1 (AOp LShift) e\<^sub>2) (parse_exp e\<^sub>1) (parse_exp e\<^sub>2)\<close> |
   \<open>\<lbrakk>length ast \<noteq> 2\<rbrakk> \<Longrightarrow> parse_exp (Node ''LSHIFT'' ast) = Error ''Expecting 2 arguments for type "LSHIFT", got many.''\<close> |
 
-  \<open>parse_exp (Node ''LOW'' [num, e]) = map_result_value2 (Cast Low) (parse_nat num) (parse_exp e)\<close> |
+  \<open>parse_exp (Node ''LOW'' [num, e]) = map_result_value2 (Cast Low) (parse_nat_dec num) (parse_exp e)\<close> |
   \<open>\<lbrakk>length ast \<noteq> 2\<rbrakk> \<Longrightarrow> parse_exp (Node ''LOW'' ast) = Error ''Expecting 2 arguments for type "LOW", got many.''\<close> |
 
-  \<open>parse_exp (Node ''HIGH'' [num, e]) = map_result_value2 (Cast High) (parse_nat num) (parse_exp e)\<close> |
+  \<open>parse_exp (Node ''HIGH'' [num, e]) = map_result_value2 (Cast High) (parse_nat_dec num) (parse_exp e)\<close> |
   \<open>\<lbrakk>length ast \<noteq> 2\<rbrakk> \<Longrightarrow> parse_exp (Node ''HIGH'' ast) = Error ''Expecting 2 arguments for type "HIGH", got many.''\<close> |
 
-  \<open>parse_exp (Node ''UNSIGNED'' [num, e]) = map_result_value2 (Cast Unsigned) (parse_nat num) (parse_exp e)\<close> |
+  \<open>parse_exp (Node ''UNSIGNED'' [num, e]) = map_result_value2 (Cast Unsigned) (parse_nat_dec num) (parse_exp e)\<close> |
   \<open>\<lbrakk>length ast \<noteq> 2\<rbrakk> \<Longrightarrow> parse_exp (Node ''UNSIGNED'' ast) = Error ''Expecting 2 arguments for type "UNSIGNED", got many.''\<close> |
 
-  \<open>parse_exp (Node ''SIGNED'' [num, e]) = map_result_value2 (Cast Signed) (parse_nat num) (parse_exp e)\<close> |
+  \<open>parse_exp (Node ''SIGNED'' [num, e]) = map_result_value2 (Cast Signed) (parse_nat_dec num) (parse_exp e)\<close> |
   \<open>\<lbrakk>length ast \<noteq> 2\<rbrakk> \<Longrightarrow> parse_exp (Node ''SIGNED'' ast) = Error ''Expecting 2 arguments for type "SIGNED", got many.''\<close> |
 
   \<open>parse_exp (Node ''Ite'' [e\<^sub>1, e\<^sub>2, e\<^sub>3]) = map_result_value3 Ite (parse_exp e\<^sub>1) (parse_exp e\<^sub>2) (parse_exp e\<^sub>3)\<close> |
@@ -166,7 +168,7 @@ where
   \<open>parse_exp (Node ''Concat'' [e\<^sub>1, e\<^sub>2]) = map_result_value2 Concat (parse_exp e\<^sub>1) (parse_exp e\<^sub>2)\<close> |
   \<open>\<lbrakk>length ast \<noteq> 2\<rbrakk> \<Longrightarrow> parse_exp (Node ''Concat'' ast) = Error ''Expecting 2 arguments for type "Concat", got many.''\<close> |
 
-  \<open>parse_exp (Node ''Extract'' [sz\<^sub>1, sz\<^sub>2, e]) = map_result_value3 Extract (parse_nat sz\<^sub>1) (parse_nat sz\<^sub>2) (parse_exp e)\<close> |
+  \<open>parse_exp (Node ''Extract'' [sz\<^sub>1, sz\<^sub>2, e]) = map_result_value3 Extract (parse_nat_dec sz\<^sub>1) (parse_nat_dec sz\<^sub>2) (parse_exp e)\<close> |
   \<open>\<lbrakk>length ast \<noteq> 3\<rbrakk> \<Longrightarrow> parse_exp (Node ''Extract'' ast) = Error ''Expecting 3 arguments for type "Extract", got many.''\<close> |
 
   \<open>\<lbrakk>e \<noteq> ''Store''; e \<noteq> ''Load''; e \<noteq> ''Var''; e \<noteq> ''Let''; e \<noteq> ''Int'';
@@ -275,19 +277,331 @@ where
   by auto
 termination by lexicographic_order
 
-definition \<open>parse_string = (parse_bil o lexer)\<close>
-(*
-record adt_trans = 
-  addr :: word
-  size :: word
-  code :: bil
+record adt_insn = 
+  adti_addr :: nat
+  adti_code :: bil
+  adti_orig :: string
 
-consts parse_adt_trans :: \<open>string \<Rightarrow> adt_trans\<close>
+fun 
+  parse_adt_insn' :: \<open>string list \<Rightarrow> adt_insn parser_result\<close>
+where
+  \<open>parse_adt_insn' lines = (
+    if (length lines = 2 \<or> length lines = 3) then
+      let 
+        lines' = if length lines = 3 then drop 1 lines else lines;
+        headers = map trim (split (CHR '':'') (lines' ! 0))
+      in 
+        map_result_value2 (\<lambda>addr bil. \<lparr> adti_addr = addr, adti_code = bil, adti_orig = (headers ! 1) \<rparr>) (nat_of_hex_string (headers ! 0)) ((parse_bil o lexer)(lines' ! 1))
+    else 
+      Error (List.append ''Expecting adt insn translation to contain two or three lines'' '''')
+  )\<close>
+
+fun 
+  parse_adt_insn :: \<open>string \<Rightarrow> adt_insn parser_result\<close>
+where
+  \<open>parse_adt_insn str = parse_adt_insn' (map trim (split LF str))\<close>
 
 lemma \<open>
-parse_adt_trans ''10450: auipc t3, 2 
-(Move(Var("X28",Imm(64)),Int(66642,64)))'' = x\<close>
+parse_adt_insn ''10450: auipc t3, 2
+(Move(Var("X28",Imm(64)),Int(66642,64)))'' 
+= Value \<lparr> 
+  adti_addr = 66640, 
+  adti_code = [Move (Var ''X28'' (Imm 64)) (Val (Immediate (Word 66642 64)))],
+  adti_orig = ''auipc t3, 2''
+\<rparr>\<close>
+  by auto
+
+record adt_function = 
+  adtf_addr :: nat
+  adtf_name :: string
+  adtf_insn :: \<open>adt_insn list\<close>
+
+fun
+  split_list :: \<open>nat \<Rightarrow> 'a list \<Rightarrow> 'a list list\<close>
+where
+  split_list_Cons: \<open>split_list n (x # xs) = (case n of 0 \<Rightarrow> [] | Suc m \<Rightarrow> (take n (x # xs)) # split_list n (drop n (x # xs)))\<close> |
+  split_list_Nil: \<open>split_list n [] = []\<close>
+
+fun
+  splitWhen :: \<open>('a \<Rightarrow> bool) \<Rightarrow> 'a list \<Rightarrow> 'a list list\<close>
+where
+  splitWhen_Cons: \<open>splitWhen P (x # xs) = (if P x then [x] # splitWhen P xs else insert_hd x (splitWhen P xs))\<close> |
+  splitWhen_Nil: \<open>splitWhen _ [] = []\<close>
+
+
+fun 
+  parse_adt_function' :: \<open>string list \<Rightarrow> adt_function parser_result\<close>
+where
+  \<open>parse_adt_function' lines = (
+      if (length lines > 2) then
+        let 
+          headers = map trim (split (CHR '':'') (lines ! 0));
+          name = tl (butlast (headers ! 1));
+          addr_result = nat_of_hex_string (headers ! 0);
+          insn_lines = drop 2 lines;
+          insn_grouped_lines = splitWhen (\<lambda>s. hd s = CHR ''('') insn_lines;
+          insn_results = map parse_adt_insn' insn_grouped_lines;
+          insns = flatten_error insn_results
+        in
+          map_result_value2 (\<lambda>addr insn. \<lparr>adtf_addr = addr, adtf_name = name, adtf_insn = insn\<rparr>) addr_result insns
+      else 
+        Error (List.append ''Expecting adt function to contain at least two lines: '' '''')
+  )\<close>
+
+fun 
+  parse_adt_function :: \<open>string \<Rightarrow> adt_function parser_result\<close>
+where
+  \<open>parse_adt_function str = parse_adt_function' (map trim (split LF str))\<close>
+
+
+lemma \<open>
+parse_adt_function 
+''10460: <setlocale>
+10460:
+10460: auipc t3, 2
+(Move(Var("X28",Imm(64)),Int(66658,64)))
+10461:
+10461: auipc t3, 2
+(Move(Var("X28",Imm(64)),Int(66658,64)))''
+= Value \<lparr>
+  adtf_addr = 66656, 
+  adtf_name = ''setlocale'',
+  adtf_insn = [\<lparr> 
+    adti_addr = 66656, 
+    adti_code = [Move (Var ''X28'' imm\<langle>64\<rangle>) (Val (Immediate (Word 66658 64)))],
+    adti_orig = ''auipc t3, 2''
+  \<rparr>, \<lparr> 
+    adti_addr = 66657, 
+    adti_code = [Move (Var ''X28'' imm\<langle>64\<rangle>) (Val (Immediate (Word 66658 64)))],
+    adti_orig = ''auipc t3, 2''
+  \<rparr>]
+\<rparr>\<close>
+  by auto
+
+
+lemma \<open>tl (butlast (''<setlocale>'')) = ''setlocale''\<close>
+  by auto
+
+
+(*
+
+10464: ld t3, -1096(t3)
+(Move(Var("X28",Imm(64)),Load(Var("mem",Mem(64,8)),PLUS(Var("X28",Imm(64)),Int(18446744073709550520,64)),LittleEndian(),64)))
+10468: jalr t1, t3
+(Move(Var("X6",Imm(64)),Int(66668,64)), Jmp(PLUS(Var("X28",Imm(64)),Int(66664,64))))
 *)
+
+record adt_section = 
+  adts_name :: string
+  adts_func :: \<open>adt_function list\<close>
+
+abbreviation \<open>section_preamble \<equiv> length ''Disassembly of section''\<close>
+
+
+fun 
+  parse_adt_section' :: \<open>string list \<Rightarrow> adt_section parser_result\<close>
+where
+  \<open>parse_adt_section' lines = (
+    let 
+      section_name = trim (drop section_preamble (lines ! 0));
+      function_lines = split [] (drop 2 lines);
+      function_results = map parse_adt_function' function_lines;
+      functions = flatten_error function_results
+    in
+      map_result_value (\<lambda>fs. \<lparr> adts_name = section_name, adts_func = fs \<rparr>) functions
+  )\<close>
+
+fun
+  parse_adt_section :: \<open>string \<Rightarrow> adt_section parser_result\<close>
+where
+  \<open>parse_adt_section str = parse_adt_section' (map trim (split LF str))\<close>
+
+lemma \<open>parse_adt_section
+''Disassembly of section .plt
+
+10450: <__libc_start_main>
+10450:
+10450: auipc t3, 2
+(Move(Var("X28",Imm(64)),Int(66642,64)))
+10454: ld t3, -1088(t3)
+(Move(Var("X28",Imm(64)),Load(Var("mem",Mem(64,8)),PLUS(Var("X28",Imm(64)),Int(18446744073709550528,64)),LittleEndian(),64)))
+10458: jalr t1, t3
+(Move(Var("X6",Imm(64)),Int(66652,64)), Jmp(PLUS(Var("X28",Imm(64)),Int(66648,64))))
+1045c:
+1045c: nop
+()
+
+10460: <setlocale>
+10460:
+10460: auipc t3, 2
+(Move(Var("X28",Imm(64)),Int(66658,64)))
+10464: ld t3, -1096(t3)
+(Move(Var("X28",Imm(64)),Load(Var("mem",Mem(64,8)),PLUS(Var("X28",Imm(64)),Int(18446744073709550520,64)),LittleEndian(),64)))
+10468: jalr t1, t3
+(Move(Var("X6",Imm(64)),Int(66668,64)), Jmp(PLUS(Var("X28",Imm(64)),Int(66664,64))))
+'' = Value \<lparr> adts_name = ''.plt'', adts_func = [\<lparr>adtf_addr = 66640,
+        adtf_name = ''__libc_start_main'',
+        adtf_insn =
+          [\<lparr>adti_addr = 66640,
+              adti_code =
+                [Var ''X28'' imm\<langle>64\<rangle> :=
+                 Val (Immediate (Word 66642 64))],
+              adti_orig = ''auipc t3, 2''\<rparr>,
+           \<lparr>adti_addr = 66644,
+              adti_code =
+                [Var ''X28'' imm\<langle>64\<rangle> :=
+                 EVar
+                  (Var ''mem''
+                    mem\<langle>64, 8\<rangle>)[BinOp
+      (EVar (Var ''X28'' imm\<langle>64\<rangle>)) (AOp Plus)
+      (Val (Immediate
+             (Word 18446744073709550528
+               64))), el]:u64],
+              adti_orig = ''ld t3, -1088(t3)''\<rparr>,
+           \<lparr>adti_addr = 66648,
+              adti_code =
+                [Var ''X6'' imm\<langle>64\<rangle> :=
+                 Val (Immediate (Word 66652 64)),
+                 jmp BinOp
+                      (EVar (Var ''X28'' imm\<langle>64\<rangle>))
+                      (AOp Plus)
+                      (Val (Immediate
+  (Word 66648 64)))],
+              adti_orig = ''jalr t1, t3''\<rparr>,
+           \<lparr>adti_addr = 66652, adti_code = [],
+              adti_orig = ''nop''\<rparr>]\<rparr>,
+     \<lparr>adtf_addr = 66656, adtf_name = ''setlocale'',
+        adtf_insn =
+          [\<lparr>adti_addr = 66656,
+              adti_code =
+                [Var ''X28'' imm\<langle>64\<rangle> :=
+                 Val (Immediate (Word 66658 64))],
+              adti_orig = ''auipc t3, 2''\<rparr>,
+           \<lparr>adti_addr = 66660,
+              adti_code =
+                [Var ''X28'' imm\<langle>64\<rangle> :=
+                 EVar
+                  (Var ''mem''
+                    mem\<langle>64, 8\<rangle>)[BinOp
+      (EVar (Var ''X28'' imm\<langle>64\<rangle>)) (AOp Plus)
+      (Val (Immediate
+             (Word 18446744073709550520
+               64))), el]:u64],
+              adti_orig = ''ld t3, -1096(t3)''\<rparr>,
+           \<lparr>adti_addr = 66664,
+              adti_code =
+                [Var ''X6'' imm\<langle>64\<rangle> :=
+                 Val (Immediate (Word 66668 64)),
+                 jmp BinOp
+                      (EVar (Var ''X28'' imm\<langle>64\<rangle>))
+                      (AOp Plus)
+                      (Val (Immediate
+  (Word 66664 64)))],
+              adti_orig = ''jalr t1, t3''\<rparr>]\<rparr>] \<rparr>\<close>
+  unfolding Let_def by auto
+
+fun 
+  parse_adt_program :: \<open>string \<Rightarrow> adt_section list parser_result\<close>
+where
+  \<open>parse_adt_program str = (
+    let 
+      lines = map trim (split LF str);
+      section_lines = splitWhile (\<lambda>s. s = ''Disassembly of section'') lines
+      section_name = trim (drop section_preamble (lines ! 0));
+      function_lines = split [] (drop 2 lines);
+      function_results = map parse_adt_function' function_lines;
+      functions = flatten_error function_results;
+      y = map_result_value (\<lambda>fs. \<lparr> adts_name = section_name, adts_func = fs \<rparr>) functions
+    in
+      Value []
+  )\<close>
+
+lemma \<open>parse_adt_program
+''
+Disassembly of section .plt
+
+10450: <__libc_start_main>
+10450:
+10450: auipc t3, 2
+(Move(Var("X28",Imm(64)),Int(66642,64)))
+10454: ld t3, -1088(t3)
+(Move(Var("X28",Imm(64)),Load(Var("mem",Mem(64,8)),PLUS(Var("X28",Imm(64)),Int(18446744073709550528,64)),LittleEndian(),64)))
+10458: jalr t1, t3
+(Move(Var("X6",Imm(64)),Int(66652,64)), Jmp(PLUS(Var("X28",Imm(64)),Int(66648,64))))
+1045c:
+1045c: nop
+()
+
+Disassembly of section .text
+
+10460: <setlocale>
+10460:
+10460: auipc t3, 2
+(Move(Var("X28",Imm(64)),Int(66658,64)))
+10464: ld t3, -1096(t3)
+(Move(Var("X28",Imm(64)),Load(Var("mem",Mem(64,8)),PLUS(Var("X28",Imm(64)),Int(18446744073709550520,64)),LittleEndian(),64)))
+10468: jalr t1, t3
+(Move(Var("X6",Imm(64)),Int(66668,64)), Jmp(PLUS(Var("X28",Imm(64)),Int(66664,64))))
+'' = Value \<lparr> adts_name = ''.plt'', adts_func = [\<lparr>adtf_addr = 66640,
+        adtf_name = ''__libc_start_main'',
+        adtf_insn =
+          [\<lparr>adti_addr = 66640,
+              adti_code =
+                [Var ''X28'' imm\<langle>64\<rangle> :=
+                 Val (Immediate (Word 66642 64))],
+              adti_orig = ''auipc t3, 2''\<rparr>,
+           \<lparr>adti_addr = 66644,
+              adti_code =
+                [Var ''X28'' imm\<langle>64\<rangle> :=
+                 EVar
+                  (Var ''mem''
+                    mem\<langle>64, 8\<rangle>)[BinOp
+      (EVar (Var ''X28'' imm\<langle>64\<rangle>)) (AOp Plus)
+      (Val (Immediate
+             (Word 18446744073709550528
+               64))), el]:u64],
+              adti_orig = ''ld t3, -1088(t3)''\<rparr>,
+           \<lparr>adti_addr = 66648,
+              adti_code =
+                [Var ''X6'' imm\<langle>64\<rangle> :=
+                 Val (Immediate (Word 66652 64)),
+                 jmp BinOp
+                      (EVar (Var ''X28'' imm\<langle>64\<rangle>))
+                      (AOp Plus)
+                      (Val (Immediate
+  (Word 66648 64)))],
+              adti_orig = ''jalr t1, t3''\<rparr>,
+           \<lparr>adti_addr = 66652, adti_code = [],
+              adti_orig = ''nop''\<rparr>]\<rparr>,
+     \<lparr>adtf_addr = 66656, adtf_name = ''setlocale'',
+        adtf_insn =
+          [\<lparr>adti_addr = 66656,
+              adti_code =
+                [Var ''X28'' imm\<langle>64\<rangle> :=
+                 Val (Immediate (Word 66658 64))],
+              adti_orig = ''auipc t3, 2''\<rparr>,
+           \<lparr>adti_addr = 66660,
+              adti_code =
+                [Var ''X28'' imm\<langle>64\<rangle> :=
+                 EVar
+                  (Var ''mem''
+                    mem\<langle>64, 8\<rangle>)[BinOp
+      (EVar (Var ''X28'' imm\<langle>64\<rangle>)) (AOp Plus)
+      (Val (Immediate
+             (Word 18446744073709550520
+               64))), el]:u64],
+              adti_orig = ''ld t3, -1096(t3)''\<rparr>,
+           \<lparr>adti_addr = 66664,
+              adti_code =
+                [Var ''X6'' imm\<langle>64\<rangle> :=
+                 Val (Immediate (Word 66668 64)),
+                 jmp BinOp
+                      (EVar (Var ''X28'' imm\<langle>64\<rangle>))
+                      (AOp Plus)
+                      (Val (Immediate
+  (Word 66664 64)))],
+              adti_orig = ''jalr t1, t3''\<rparr>]\<rparr>] \<rparr>\<close>
+  unfolding Let_def by auto
 
 
 end
