ExpressionSemantics/Expression_Intros.thy
@@ -30,10 +30,10 @@ lemmas step_load_un_memI = LoadUnMem
 lemmas step_load_word_beI = LoadWordBe
 lemmas step_load_word_elI = LoadWordEl
 
-interpretation step_load_memI: exp_syntax \<open>\<lambda>e. (\<And>\<Delta> e\<^sub>1 e\<^sub>1' ed sz. \<Delta> \<turnstile> e\<^sub>1 \<leadsto> e\<^sub>1' \<Longrightarrow> \<Delta> \<turnstile> e\<^sub>1[e, ed]:usz \<leadsto> (e\<^sub>1'[e, ed]:usz))\<close>
+interpretation step_load_memI: exp_val_syntax \<open>\<lambda>e _. (\<And>\<Delta> e\<^sub>1 e\<^sub>1' ed sz. \<Delta> \<turnstile> e\<^sub>1 \<leadsto> e\<^sub>1' \<Longrightarrow> \<Delta> \<turnstile> e\<^sub>1[e, ed]:usz \<leadsto> (e\<^sub>1'[e, ed]:usz))\<close>
   by (standard, rule step_load_memI)
 
-interpretation step_load_un_memI: exp_syntax \<open>\<lambda>e. (\<And>\<Delta> str t ed sz. \<Delta> \<turnstile> (unknown[str]: t)[e, ed]:usz \<leadsto> unknown[str]: imm\<langle>sz\<rangle>)\<close>
+interpretation step_load_un_memI: exp_val_syntax \<open>\<lambda>e _. (\<And>\<Delta> str t ed sz. \<Delta> \<turnstile> (unknown[str]: t)[e, ed]:usz \<leadsto> unknown[str]: imm\<langle>sz\<rangle>)\<close>
   by (standard, rule step_load_un_memI)
 
 interpretation step_load_byteI: word_exp_val_syntax \<open>\<lambda>w\<^sub>w w\<^sub>e _ e v'. (\<And>\<Delta> v sz ed. \<Delta> \<turnstile> v[w\<^sub>w \<leftarrow> v', sz][w\<^sub>e, ed]:usz \<leadsto> e)\<close>
@@ -50,57 +50,25 @@ interpretation step_load_word_beI: load_multiple_syntax \<open>\<lambda>e\<^sub>
 interpretation step_load_word_elI: load_multiple_syntax \<open>\<lambda>e\<^sub>1 v\<^sub>1 sz\<^sub>a\<^sub>d\<^sub>d\<^sub>r sz\<^sub>m\<^sub>e\<^sub>m e\<^sub>w. (\<And>\<Delta> sz. sz\<^sub>m\<^sub>e\<^sub>m < sz \<Longrightarrow>
 \<Delta> \<turnstile> e\<^sub>1[e\<^sub>w, el]:usz \<leadsto> (e\<^sub>1[succ e\<^sub>w, el]:usz - sz\<^sub>m\<^sub>e\<^sub>m @ (e\<^sub>1[e\<^sub>w, el]:usz\<^sub>m\<^sub>e\<^sub>m)))\<close>
   by (standard, rule step_load_word_elI)
-(*
-lemma LOAD_WORD_EL_MEM_INTER: (* TODO *)
-  assumes \<open>sz\<^sub>m\<^sub>e\<^sub>m < sz\<close> and \<open>\<exists>num. w = (num \<Colon> sz\<^sub>a\<^sub>d\<^sub>d\<^sub>r)\<close>
-    shows \<open>\<Delta> \<turnstile> (v[w \<leftarrow> num\<^sub>2 \<Colon> sz\<^sub>m\<^sub>e\<^sub>m, sz\<^sub>m\<^sub>e\<^sub>m][(num \<Colon> sz\<^sub>a\<^sub>d\<^sub>d\<^sub>r), el]:usz) \<leadsto> (((v[w \<leftarrow> num\<^sub>2 \<Colon> sz\<^sub>m\<^sub>e\<^sub>m, sz\<^sub>m\<^sub>e\<^sub>m][succ (num \<Colon> sz\<^sub>a\<^sub>d\<^sub>d\<^sub>r), el]:u(sz - sz\<^sub>m\<^sub>e\<^sub>m))) @ (v[w \<leftarrow> num\<^sub>2 \<Colon> sz\<^sub>m\<^sub>e\<^sub>m, sz\<^sub>m\<^sub>e\<^sub>m][(num \<Colon> sz\<^sub>a\<^sub>d\<^sub>d\<^sub>r), el]:usz\<^sub>m\<^sub>e\<^sub>m))\<close> 
-  using assms(2) apply auto
-  using assms(1) by (rule step_load_word_el.storageI)
 
-
-lemmas LOAD_WORD_EL_MEM = step_load_word_el.storageI (* TODO *)
-
-lemma LOAD_WORD_EL_MEM_SUCC: (* TODO *)
-  assumes \<open>sz\<^sub>m\<^sub>e\<^sub>m < sz\<close>
-    shows \<open>\<Delta> \<turnstile> (v[succ (num\<^sub>1 \<Colon> sz\<^sub>a\<^sub>d\<^sub>d\<^sub>r) \<leftarrow> num\<^sub>2 \<Colon> sz\<^sub>m\<^sub>e\<^sub>m, sz\<^sub>m\<^sub>e\<^sub>m][(num \<Colon> sz\<^sub>a\<^sub>d\<^sub>d\<^sub>r), el]:usz) \<leadsto> (((v[succ (num\<^sub>1 \<Colon> sz\<^sub>a\<^sub>d\<^sub>d\<^sub>r) \<leftarrow> num\<^sub>2 \<Colon> sz\<^sub>m\<^sub>e\<^sub>m, sz\<^sub>m\<^sub>e\<^sub>m][succ (num \<Colon> sz\<^sub>a\<^sub>d\<^sub>d\<^sub>r), el]:u(sz - sz\<^sub>m\<^sub>e\<^sub>m))) @ (v[succ (num\<^sub>1 \<Colon> sz\<^sub>a\<^sub>d\<^sub>d\<^sub>r) \<leftarrow> num\<^sub>2 \<Colon> sz\<^sub>m\<^sub>e\<^sub>m, sz\<^sub>m\<^sub>e\<^sub>m][(num \<Colon> sz\<^sub>a\<^sub>d\<^sub>d\<^sub>r), el]:usz\<^sub>m\<^sub>e\<^sub>m))\<close> 
-  using assms 
-  unfolding succ.simps(1)[of num\<^sub>1 sz\<^sub>a\<^sub>d\<^sub>d\<^sub>r] bv_plus.simps
-  by (rule LOAD_WORD_EL_MEM)
-
-lemma LOAD_WORD_EL_MEM_SUCC2:(* TODO *)
-  assumes \<open>sz\<^sub>m\<^sub>e\<^sub>m < sz\<close>
-    shows \<open>\<Delta> \<turnstile> (v[succ (succ (num\<^sub>1 \<Colon> sz\<^sub>a\<^sub>d\<^sub>d\<^sub>r)) \<leftarrow> num\<^sub>2 \<Colon> sz\<^sub>m\<^sub>e\<^sub>m, sz\<^sub>m\<^sub>e\<^sub>m][(num \<Colon> sz\<^sub>a\<^sub>d\<^sub>d\<^sub>r), el]:usz) \<leadsto> (((v[succ (succ (num\<^sub>1 \<Colon> sz\<^sub>a\<^sub>d\<^sub>d\<^sub>r)) \<leftarrow> num\<^sub>2 \<Colon> sz\<^sub>m\<^sub>e\<^sub>m, sz\<^sub>m\<^sub>e\<^sub>m][succ (num \<Colon> sz\<^sub>a\<^sub>d\<^sub>d\<^sub>r), el]:u(sz - sz\<^sub>m\<^sub>e\<^sub>m))) @ (v[succ (succ (num\<^sub>1 \<Colon> sz\<^sub>a\<^sub>d\<^sub>d\<^sub>r)) \<leftarrow> num\<^sub>2 \<Colon> sz\<^sub>m\<^sub>e\<^sub>m, sz\<^sub>m\<^sub>e\<^sub>m][(num \<Colon> sz\<^sub>a\<^sub>d\<^sub>d\<^sub>r), el]:usz\<^sub>m\<^sub>e\<^sub>m))\<close> 
-  using assms 
-  unfolding succ.simps(1)[of num\<^sub>1 sz\<^sub>a\<^sub>d\<^sub>d\<^sub>r] bv_plus.simps
-  by (rule LOAD_WORD_EL_MEM_SUCC)
-
-lemma LOAD_WORD_EL_MEM_SUCC3:(* TODO *)
-  assumes \<open>sz\<^sub>m\<^sub>e\<^sub>m < sz\<close>
-    shows \<open>\<Delta> \<turnstile> (v[succ (succ (succ (num\<^sub>1 \<Colon> sz\<^sub>a\<^sub>d\<^sub>d\<^sub>r))) \<leftarrow> num\<^sub>2 \<Colon> sz\<^sub>m\<^sub>e\<^sub>m, sz\<^sub>m\<^sub>e\<^sub>m][(num \<Colon> sz\<^sub>a\<^sub>d\<^sub>d\<^sub>r), el]:usz) \<leadsto> (((v[succ (succ (succ (num\<^sub>1 \<Colon> sz\<^sub>a\<^sub>d\<^sub>d\<^sub>r))) \<leftarrow> num\<^sub>2 \<Colon> sz\<^sub>m\<^sub>e\<^sub>m, sz\<^sub>m\<^sub>e\<^sub>m][succ (num \<Colon> sz\<^sub>a\<^sub>d\<^sub>d\<^sub>r), el]:u(sz - sz\<^sub>m\<^sub>e\<^sub>m))) @ (v[succ (succ (succ (num\<^sub>1 \<Colon> sz\<^sub>a\<^sub>d\<^sub>d\<^sub>r))) \<leftarrow> num\<^sub>2 \<Colon> sz\<^sub>m\<^sub>e\<^sub>m, sz\<^sub>m\<^sub>e\<^sub>m][(num \<Colon> sz\<^sub>a\<^sub>d\<^sub>d\<^sub>r), el]:usz\<^sub>m\<^sub>e\<^sub>m))\<close> 
-  using assms 
-  unfolding succ.simps(1)[of num\<^sub>1 sz\<^sub>a\<^sub>d\<^sub>d\<^sub>r] bv_plus.simps
-  by (rule LOAD_WORD_EL_MEM_SUCC2)
-
-lemmas LOAD_WORD_EL_MEM_WORD_ADDR = step_load_word_el.storageI (* TODO *)
-*)
 subsection \<open>Stores\<close>
 
 lemmas step_store_step_valI = StoreStepVal
-lemmas step_store_addrI = StoreStepAddr
-lemmas step_store_memI = StoreStepMem
-lemmas step_store_valI = StoreVal
-lemmas step_store_un_addrI = StoreUnAddr
 
-interpretation step_store_addrI: exp_syntax \<open>\<lambda>e. (\<And>\<Delta> e\<^sub>1 e\<^sub>1' e\<^sub>2 e\<^sub>2' en sz. \<Delta> \<turnstile> e\<^sub>2 \<leadsto> e\<^sub>2' \<Longrightarrow> \<Delta> \<turnstile> e\<^sub>1 with [e\<^sub>2, en]:usz \<leftarrow> e \<leadsto> (e\<^sub>1 with [e\<^sub>2', en]:usz \<leftarrow> e))\<close>
+lemmas step_store_addrI = StoreStepAddr
+interpretation step_store_addrI: exp_val_syntax \<open>\<lambda>e _. (\<And>\<Delta> e\<^sub>1 e\<^sub>1' e\<^sub>2 e\<^sub>2' en sz. \<Delta> \<turnstile> e\<^sub>2 \<leadsto> e\<^sub>2' \<Longrightarrow> \<Delta> \<turnstile> e\<^sub>1 with [e\<^sub>2, en]:usz \<leftarrow> e \<leadsto> (e\<^sub>1 with [e\<^sub>2', en]:usz \<leftarrow> e))\<close>
   by (standard, rule step_store_addrI)
 
+lemmas step_store_un_addrI = StoreUnAddr
 interpretation step_store_un_addrI: exp2_val_syntax \<open>\<lambda>e\<^sub>1 e\<^sub>2 v\<^sub>1 _. (\<And>\<Delta> t t' str ed sz. type v\<^sub>1 = t \<Longrightarrow> \<Delta> \<turnstile> e\<^sub>1 with [unknown[str]: t', ed]:usz \<leftarrow> e\<^sub>2 \<leadsto> unknown[str]: t)\<close>
   by (standard, rule step_store_un_addrI)
 
+lemmas step_store_memI = StoreStepMem
 interpretation step_store_memI: exp2_val_syntax \<open>\<lambda>e\<^sub>1 e\<^sub>2 _ _. (\<And>\<Delta> e e' en sz. \<Delta> \<turnstile> e \<leadsto> e' \<Longrightarrow> \<Delta> \<turnstile> e with [e\<^sub>1, en]:usz \<leftarrow> e\<^sub>2 \<leadsto> (e' with [e\<^sub>1, en]:usz \<leftarrow> e\<^sub>2))\<close>
   by (standard, rule step_store_memI)
 
-interpretation step_store_valI: exp2_storage_val_syntax \<open>\<lambda>e\<^sub>1 e\<^sub>2 v\<^sub>1 v\<^sub>2 sz\<^sub>a\<^sub>d\<^sub>d\<^sub>r sz\<^sub>m\<^sub>e\<^sub>m. (\<And>\<Delta> num en. \<Delta> \<turnstile> e\<^sub>1 with [num \<Colon> sz\<^sub>a\<^sub>d\<^sub>d\<^sub>r, en]:usz\<^sub>m\<^sub>e\<^sub>m \<leftarrow> e\<^sub>2 \<leadsto> (v\<^sub>1[num \<Colon> sz\<^sub>a\<^sub>d\<^sub>d\<^sub>r \<leftarrow> v\<^sub>2, sz\<^sub>m\<^sub>e\<^sub>m]))\<close>
+lemmas step_store_valI = StoreVal
+interpretation step_store_valI: store_multiple_syntax \<open>\<lambda>e\<^sub>1 v\<^sub>1 e\<^sub>2 _ w\<^sub>2 e\<^sub>3 v\<^sub>3 sz\<^sub>a\<^sub>d\<^sub>d\<^sub>r sz\<^sub>m\<^sub>e\<^sub>m. (\<And>\<Delta> en. \<Delta> \<turnstile> e\<^sub>1 with [e\<^sub>2, en]:usz\<^sub>m\<^sub>e\<^sub>m \<leftarrow> e\<^sub>3 \<leadsto> (v\<^sub>1[w\<^sub>2 \<leftarrow> v\<^sub>3, sz\<^sub>m\<^sub>e\<^sub>m]))\<close>
   by (standard, rule step_store_valI)
 
 lemmas step_store_word_beI = StoreWordBe
@@ -114,45 +82,7 @@ interpretation step_store_word_elI: exp2_storage_val_syntax \<open>\<lambda>e\<^
    e = e\<^sub>1 with [num \<Colon> sz\<^sub>a\<^sub>d\<^sub>d\<^sub>r, el]:usz\<^sub>m\<^sub>e\<^sub>m \<leftarrow> (low:sz\<^sub>m\<^sub>e\<^sub>m[e\<^sub>2])\<rbrakk> \<Longrightarrow>
 \<Delta> \<turnstile> e\<^sub>1 with [num \<Colon> sz\<^sub>a\<^sub>d\<^sub>d\<^sub>r, el]:usz \<leftarrow> e\<^sub>2 \<leadsto> (e with [succ (num \<Colon> sz\<^sub>a\<^sub>d\<^sub>d\<^sub>r), el]:usz - sz\<^sub>m\<^sub>e\<^sub>m \<leftarrow> (high:sz - sz\<^sub>m\<^sub>e\<^sub>m[e\<^sub>2])))\<close>
   by (standard, rule step_store_word_elI)
-(*
-lemmas STORE_STEP_MEM_WORD = step_store_mem.word.wordI (* TODO *)
 
-lemmas STORE_WORD_EL_WORD = step_store_word_el.val.wordI (* TODO *)
-
-lemmas STORE_WORD_EL_WORD_MEM = step_store_word_el.storage.wordI (* TODO *)
-
-lemmas STORE_WORD = step_store_val.val.wordI (* TODO *)
-
-lemmas STORE_WORD_IN_MEM = step_store_val.storage.wordI (* TODO *)
-
-lemma STORE_STEP_MEM_BV_ADD: (* TODO *)
-  assumes \<open>\<Delta> \<turnstile> e\<^sub>1 \<leadsto> e\<^sub>1'\<close>
-    shows \<open>\<Delta> \<turnstile> e\<^sub>1 with [(num\<^sub>2 \<Colon> sz\<^sub>2) +\<^sub>b\<^sub>v (num\<^sub>3 \<Colon> sz\<^sub>2), en]:usz \<leftarrow> (num\<^sub>4 \<Colon> sz\<^sub>4) \<leadsto> e\<^sub>1' with [(num\<^sub>2 \<Colon> sz\<^sub>2) +\<^sub>b\<^sub>v (num\<^sub>3 \<Colon> sz\<^sub>2), en]:usz \<leftarrow> (num\<^sub>4 \<Colon> sz\<^sub>4)\<close>
-  using assms unfolding bv_plus.simps by (rule STORE_STEP_MEM_WORD)
-
-lemma STORE_STEP_MEM_SUCC: (* TODO *)
-  assumes \<open>\<Delta> \<turnstile> e\<^sub>1 \<leadsto> e\<^sub>1'\<close>
-    shows \<open>\<Delta> \<turnstile> e\<^sub>1 with [succ (num\<^sub>2 \<Colon> sz\<^sub>2), en]:usz \<leftarrow> (num\<^sub>3 \<Colon> sz\<^sub>3) \<leadsto> e\<^sub>1' with [succ (num\<^sub>2 \<Colon> sz\<^sub>2), en]:usz \<leftarrow> (num\<^sub>3 \<Colon> sz\<^sub>3)\<close>
-  using assms unfolding succ.simps by (rule STORE_STEP_MEM_BV_ADD)
-
-lemma STORE_STEP_MEM_SUCC_XTRACT: (* TODO *)
-  assumes \<open>\<Delta> \<turnstile> e\<^sub>1 \<leadsto> e\<^sub>1'\<close>
-    shows \<open>\<Delta> \<turnstile> e\<^sub>1 with [succ (num\<^sub>2 \<Colon> sz\<^sub>2), en]:usz \<leftarrow> ext (num\<^sub>3 \<Colon> sz\<^sub>3) \<sim> hi : sz' \<sim> lo : sz'' \<leadsto> e\<^sub>1' with [succ (num\<^sub>2 \<Colon> sz\<^sub>2), en]:usz \<leftarrow> ext (num\<^sub>3 \<Colon> sz\<^sub>3) \<sim> hi : sz' \<sim> lo : sz''\<close>
-  using assms unfolding xtract.simps by (rule STORE_STEP_MEM_SUCC)
-
-lemma STORE_XTRACT: (* TODO *)
-  assumes \<open>sz\<^sub>m\<^sub>e\<^sub>m > 0\<close> and \<open>sz\<^sub>m\<^sub>e\<^sub>m = sz\<^sub>2 - sz\<^sub>3 + 1\<close> and \<open>type v = mem\<langle>sz\<^sub>a\<^sub>d\<^sub>d\<^sub>r, sz\<^sub>m\<^sub>e\<^sub>m\<rangle>\<close>
-    shows \<open>\<Delta> \<turnstile> (Val v with [(num \<Colon> sz\<^sub>a\<^sub>d\<^sub>d\<^sub>r), ed]:usz\<^sub>m\<^sub>e\<^sub>m \<leftarrow> ext (num\<^sub>v\<^sub>a\<^sub>l \<Colon> sz\<^sub>1) \<sim> hi : sz\<^sub>2 \<sim> lo : sz\<^sub>3) \<leadsto> (v[(num \<Colon> sz\<^sub>a\<^sub>d\<^sub>d\<^sub>r) \<leftarrow> ext (num\<^sub>v\<^sub>a\<^sub>l \<Colon> sz\<^sub>1) \<sim> hi : sz\<^sub>2 \<sim> lo : sz\<^sub>3, sz\<^sub>m\<^sub>e\<^sub>m])\<close>
-  unfolding xtract.simps assms(2)[symmetric]
-  apply (rule STORE_WORD)
-  using assms(1,3) by blast+
-
-lemma STORE_XTRACT_IN_MEM: (* TODO *)
-  assumes \<open>sz\<^sub>m\<^sub>e\<^sub>m > 0\<close> and \<open>sz\<^sub>m\<^sub>e\<^sub>m = sz\<^sub>2 - sz\<^sub>3 + 1\<close>
-    shows \<open>\<Delta> \<turnstile> (v[numa \<Colon> sz\<^sub>a\<^sub>d\<^sub>d\<^sub>r \<leftarrow> numv \<Colon> sz\<^sub>m\<^sub>e\<^sub>m, sz\<^sub>m\<^sub>e\<^sub>m] with [(num \<Colon> sz\<^sub>a\<^sub>d\<^sub>d\<^sub>r), ed]:usz\<^sub>m\<^sub>e\<^sub>m \<leftarrow> ext (num\<^sub>v\<^sub>a\<^sub>l \<Colon> sz\<^sub>1) \<sim> hi : sz\<^sub>2 \<sim> lo : sz\<^sub>3) \<leadsto> (v[numa \<Colon> sz\<^sub>a\<^sub>d\<^sub>d\<^sub>r \<leftarrow> numv \<Colon> sz\<^sub>m\<^sub>e\<^sub>m, sz\<^sub>m\<^sub>e\<^sub>m][(num \<Colon> sz\<^sub>a\<^sub>d\<^sub>d\<^sub>r) \<leftarrow> ext (num\<^sub>v\<^sub>a\<^sub>l \<Colon> sz\<^sub>1) \<sim> hi : sz\<^sub>2 \<sim> lo : sz\<^sub>3, sz\<^sub>m\<^sub>e\<^sub>m])\<close>
-  using assms(1) unfolding xtract.simps assms(2)[symmetric]
-  by (rule STORE_WORD_IN_MEM)
-*)
 subsection \<open>Let\<close>
 
 lemmas step_let_stepI = LetStep
@@ -170,7 +100,7 @@ lemmas step_ite_trueI = IfTrue
 lemmas step_ite_falseI = IfFalse
 lemmas step_ite_unI = IfUnknown
 
-interpretation step_ite_thenI: exp_syntax \<open>\<lambda>e. (\<And>\<Delta> e\<^sub>1 e\<^sub>1' e\<^sub>2 e\<^sub>2'. \<Delta> \<turnstile> e\<^sub>2 \<leadsto> e\<^sub>2' \<Longrightarrow> \<Delta> \<turnstile> ite e\<^sub>1 e\<^sub>2 e \<leadsto> ite e\<^sub>1 e\<^sub>2' e)\<close>
+interpretation step_ite_thenI: exp_val_syntax \<open>\<lambda>e _. (\<And>\<Delta> e\<^sub>1 e\<^sub>1' e\<^sub>2 e\<^sub>2'. \<Delta> \<turnstile> e\<^sub>2 \<leadsto> e\<^sub>2' \<Longrightarrow> \<Delta> \<turnstile> ite e\<^sub>1 e\<^sub>2 e \<leadsto> ite e\<^sub>1 e\<^sub>2' e)\<close>
   by (standard, rule step_ite_thenI)
 
 interpretation step_ite_condI: exp2_val_syntax \<open>\<lambda>e\<^sub>1 e\<^sub>2 _ _. (\<And>\<Delta> e e'. \<Delta> \<turnstile> e \<leadsto> e' \<Longrightarrow> \<Delta> \<turnstile> ite e e\<^sub>1 e\<^sub>2 \<leadsto> ite e' e\<^sub>1 e\<^sub>2)\<close>
@@ -191,7 +121,7 @@ subsection \<open>Bop\<close>
 lemmas step_bop_lhsI = BopLhs
 lemmas step_bop_rhsI = BopRhs
 
-interpretation step_bop_rhsI: exp_syntax \<open>\<lambda>e. (\<And>\<Delta> e\<^sub>2 bop e\<^sub>2'. \<Delta> \<turnstile> e\<^sub>2 \<leadsto> e\<^sub>2' \<Longrightarrow> \<Delta> \<turnstile> BinOp e bop e\<^sub>2 \<leadsto> BinOp e bop e\<^sub>2')\<close>
+interpretation step_bop_rhsI: exp_val_syntax \<open>\<lambda>e _. (\<And>\<Delta> e\<^sub>2 bop e\<^sub>2'. \<Delta> \<turnstile> e\<^sub>2 \<leadsto> e\<^sub>2' \<Longrightarrow> \<Delta> \<turnstile> BinOp e bop e\<^sub>2 \<leadsto> BinOp e bop e\<^sub>2')\<close>
   by (standard, rule step_bop_rhsI)
 
 locale bop_lemmas =
@@ -204,7 +134,7 @@ lemma lhsI:
     shows \<open>\<Delta> \<turnstile> bop_fun e\<^sub>1 e\<^sub>2 \<leadsto> bop_fun e\<^sub>1' e\<^sub>2\<close>
   using assms unfolding bop_simps by (rule step_bop_lhsI)
 
-sublocale rhs: exp_syntax \<open>\<lambda>e. (\<And>\<Delta> e\<^sub>2 e\<^sub>2'. \<Delta> \<turnstile> e\<^sub>2 \<leadsto> e\<^sub>2' \<Longrightarrow> \<Delta> \<turnstile> bop_fun e e\<^sub>2 \<leadsto> bop_fun e e\<^sub>2')\<close>
+sublocale rhs: exp_val_syntax \<open>\<lambda>e _. (\<And>\<Delta> e\<^sub>2 e\<^sub>2'. \<Delta> \<turnstile> e\<^sub>2 \<leadsto> e\<^sub>2' \<Longrightarrow> \<Delta> \<turnstile> bop_fun e e\<^sub>2 \<leadsto> bop_fun e e\<^sub>2')\<close>
   apply standard
   unfolding bop_simps by (rule step_bop_rhsI)
 
@@ -322,19 +252,19 @@ subsection \<open>Concat\<close>
 lemmas step_concat_rhsI = ConcatRhs
 
 lemmas step_concatI = Concat
-interpretation step_concatI: exp2_val_is_word_syntax \<open>\<lambda>e\<^sub>1 _ e\<^sub>2 _. (\<And>\<Delta>. \<Delta> \<turnstile> (e\<^sub>1 @ e\<^sub>2) \<leadsto> (e\<^sub>1 \<cdot> e\<^sub>2))\<close>
+interpretation step_concatI: exp2_val_word_sz_syntax \<open>\<lambda>e\<^sub>1 _ _ _ e\<^sub>2 _ _ _. (\<And>\<Delta>. \<Delta> \<turnstile> (e\<^sub>1 @ e\<^sub>2) \<leadsto> (e\<^sub>1 \<cdot> e\<^sub>2))\<close>
   by (standard, rule step_concatI)
 
 lemmas step_concat_lhsI = ConcatLhs
-interpretation step_concat_lhsI: exp_syntax \<open>\<lambda>e. (\<And>\<Delta> e\<^sub>1 e\<^sub>1'. \<Delta> \<turnstile> e\<^sub>1 \<leadsto> e\<^sub>1' \<Longrightarrow> \<Delta> \<turnstile> (e\<^sub>1 @ e) \<leadsto> (e\<^sub>1' @ e))\<close>
+interpretation step_concat_lhsI: exp_val_syntax \<open>\<lambda>e _. (\<And>\<Delta> e\<^sub>1 e\<^sub>1'. \<Delta> \<turnstile> e\<^sub>1 \<leadsto> e\<^sub>1' \<Longrightarrow> \<Delta> \<turnstile> (e\<^sub>1 @ e) \<leadsto> (e\<^sub>1' @ e))\<close>
   by (standard, rule step_concat_lhsI)
 
 lemmas step_concat_lhs_unI = ConcatLhsUn
-interpretation step_concat_lhs_unI: exp_word_syntax \<open>\<lambda>e v sz. (\<And>\<Delta> sz\<^sub>1 str. \<Delta> \<turnstile> ((unknown[str]: imm\<langle>sz\<^sub>1\<rangle>) @ e) \<leadsto> unknown[str]: imm\<langle>sz\<^sub>1 + sz\<rangle>)\<close>
+interpretation step_concat_lhs_unI: exp_val_is_imm_syntax \<open>\<lambda>e v sz. (\<And>\<Delta> sz\<^sub>1 str. \<Delta> \<turnstile> ((unknown[str]: imm\<langle>sz\<^sub>1\<rangle>) @ e) \<leadsto> unknown[str]: imm\<langle>sz\<^sub>1 + sz\<rangle>)\<close>
   by (standard, rule step_concat_lhs_unI)
 
 lemmas step_concat_rhs_unI = ConcatRhsUn
-interpretation step_concat_rhs_unI: exp_word_syntax \<open>\<lambda>e v sz. (\<And>\<Delta> sz\<^sub>2 str. \<Delta> \<turnstile> (e @ unknown[str]: imm\<langle>sz\<^sub>2\<rangle>) \<leadsto> unknown[str]: imm\<langle>sz + sz\<^sub>2\<rangle>)\<close>
+interpretation step_concat_rhs_unI: exp_val_is_imm_syntax \<open>\<lambda>e v sz. (\<And>\<Delta> sz\<^sub>2 str. \<Delta> \<turnstile> (e @ unknown[str]: imm\<langle>sz\<^sub>2\<rangle>) \<leadsto> unknown[str]: imm\<langle>sz + sz\<^sub>2\<rangle>)\<close>
   by (standard, rule step_concat_rhs_unI)
 
 subsection \<open>Extract\<close>
@@ -348,9 +278,20 @@ subsection \<open>Cast\<close>
 lemmas step_cast_reduceI = CastReduce
 lemmas step_cast_unkI = CastUnk
 lemmas step_cast_lowI = CastLow
+interpretation step_cast_lowI: exp_val_word_sz_syntax \<open>\<lambda>e _ _ _. (\<And>\<Delta> sz. \<Delta> \<turnstile> low:sz[e] \<leadsto> ext e \<sim> hi : sz - 1 \<sim> lo : 0)\<close>
+  by (standard, rule step_cast_lowI)
+
 lemmas step_cast_highI = CastHigh
-lemmas step_cast_signedI = CastSigned
+interpretation step_cast_highI: exp_val_word_sz_syntax \<open>\<lambda>e _ _ sz'. (\<And>\<Delta> sz. \<Delta> \<turnstile> high:sz[e] \<leadsto> ext e \<sim> hi : sz' - 1 \<sim> lo : sz' - sz)\<close>
+  by (standard, rule step_cast_highI)
+
+lemmas step_cast_signedI = CastSigned 
+interpretation step_cast_signedI: exp_val_word_sz_syntax \<open>\<lambda>e _ _ _. (\<And>\<Delta> sz. \<Delta> \<turnstile> extend:sz[e] \<leadsto> ext e \<sim> hi : sz - 1 \<sim> lo : 0)\<close>
+  by (standard, rule step_cast_signedI)
+
 lemmas step_cast_unsignedI = CastUnsigned
+interpretation step_cast_unsignedI: exp_val_word_sz_syntax \<open>\<lambda>e _ _ _. (\<And>\<Delta> sz. \<Delta> \<turnstile> pad:sz[e] \<leadsto> ext e \<sim> hi : sz - 1 \<sim> lo : 0)\<close>
+  by (standard, rule step_cast_unsignedI)
 
 (* TODO move *)
 
@@ -361,38 +302,7 @@ lemmas solve_exp_simpset = (*mod_mod_trivial*) mod_Suc_eq not_dvd_plus_mod_neq n
 
 method solve_word_neq = (simp (no_asm) add: solve_exp_simpset succ.simps bv_plus.simps; fail)
 method solve_bv_neqI = (rule bv_not_eq_same_sz_true, (simp; fail))
-
-method solve_expI = (
-    \<comment> \<open>Attempt to discharge trivial rules (non assumptions)\<close>
-  intro step_load_un_memI.syntaxs
-  step_store_valI.storage.syntaxs step_store_valI.unknown.syntaxs
-   
-  step_letI.syntaxs
-  step_ite_trueI.syntaxs2  step_ite_falseI.syntaxs2
-
-  step_plusI step_plusI.unk_lhsI step_plusI.unk_rhsI
-  step_minusI step_minusI.unk_lhsI step_minusI.unk_rhsI
-  step_timesI step_timesI.unk_lhsI step_timesI.unk_rhsI 
-  step_divI step_divideI.unk_lhsI step_divideI.unk_rhsI 
-  step_sdivI step_sdivideI.unk_lhsI step_sdivideI.unk_rhsI 
-  step_modI step_modI.unk_lhsI step_modI.unk_rhsI 
-  step_smodI step_smodI.unk_lhsI step_smodI.unk_rhsI 
-  step_lslI step_lslI.unk_lhsI step_lslI.unk_rhsI 
-  step_lsrI step_lsrI.unk_lhsI step_lsrI.unk_rhsI
-  step_asrI step_asrI.unk_lhsI step_asrI.unk_rhsI
-  step_landI step_landI.unk_lhsI step_landI.unk_rhsI
-  step_lorI step_lorI.unk_lhsI step_lorI.unk_rhsI
-  step_xorI step_xorI.unk_lhsI step_xorI.unk_rhsI
-  step_eq_sameI step_neq_sameI 
-  step_lessI step_ltI.unk_lhsI step_ltI.unk_rhsI
-  step_less_eqI step_leI.unk_lhsI step_leI.unk_rhsI
-  step_signed_lessI step_sltI.unk_lhsI step_sltI.unk_rhsI
-  step_signed_less_eqI step_sleI.unk_lhsI step_sleI.unk_rhsI
-  step_lop_unk_lhsI step_lop_unk_rhsI step_aop_unk_rhsI step_aop_unk_lhsI
-
-  step_concat_lhs_unI.word_syntaxs step_concat_rhs_unI.word_syntaxs
-  
-  |
+method solve_expI uses simp = (((unfold simp)?), (
 
   \<comment> \<open>Vars\<close>
   (rule step_var_inI.word, solve_in_var) |
@@ -402,39 +312,67 @@ method solve_expI = (
   \<comment> \<open>Loads\<close>
   rule step_load_un_addrI |
 
-  rule step_load_byteI.word.word | rule step_load_byteI.word.true | rule step_load_byteI.word.false | rule step_load_byteI.word.storage | rule step_load_byteI.word.unknown | rule step_load_byteI.word.xtract |
-  rule step_load_byteI.word.succ | rule step_load_byteI.word.succ2 | rule step_load_byteI.word.succ3 | rule step_load_byteI.word.succ4 | rule step_load_byteI.word.succ5 | rule step_load_byteI.word.succ6 | rule step_load_byteI.word.succ7 |
+  rule step_load_byteI.word.word | rule step_load_byteI.word.true | rule step_load_byteI.word.false | 
+  rule step_load_byteI.word.storage | 
+  rule step_load_byteI.word.unknown | rule step_load_byteI.word.xtract |
+  rule step_load_byteI.word.succ | rule step_load_byteI.word.succ2 | rule step_load_byteI.word.succ3 | 
+  rule step_load_byteI.word.succ4 | rule step_load_byteI.word.succ5 | rule step_load_byteI.word.succ6 | 
+  rule step_load_byteI.word.succ7 |
   rule step_load_byteI.word.val |
 
-  rule step_load_byteI.succ.word | rule step_load_byteI.succ.true | rule step_load_byteI.succ.false | rule step_load_byteI.succ.storage | rule step_load_byteI.succ.unknown | rule step_load_byteI.succ.xtract |
-  rule step_load_byteI.succ.succ | rule step_load_byteI.succ.succ2 | rule step_load_byteI.succ.succ3 | rule step_load_byteI.succ.succ4 | rule step_load_byteI.succ.succ5 | rule step_load_byteI.succ.succ6 | rule step_load_byteI.succ.succ7 |
+  rule step_load_byteI.succ.word | rule step_load_byteI.succ.true | rule step_load_byteI.succ.false | 
+  rule step_load_byteI.succ.storage | 
+  rule step_load_byteI.succ.unknown | rule step_load_byteI.succ.xtract |
+  rule step_load_byteI.succ.succ | rule step_load_byteI.succ.succ2 | rule step_load_byteI.succ.succ3 | 
+  rule step_load_byteI.succ.succ4 | rule step_load_byteI.succ.succ5 | rule step_load_byteI.succ.succ6 | 
+  rule step_load_byteI.succ.succ7 |
   rule step_load_byteI.succ.val |
 
-  rule step_load_byteI.succ2.word | rule step_load_byteI.succ2.true | rule step_load_byteI.succ2.false | rule step_load_byteI.succ2.storage | rule step_load_byteI.succ2.unknown | rule step_load_byteI.succ2.xtract |
-  rule step_load_byteI.succ2.succ | rule step_load_byteI.succ2.succ2 | rule step_load_byteI.succ2.succ3 | rule step_load_byteI.succ2.succ4 | rule step_load_byteI.succ2.succ5 | rule step_load_byteI.succ2.succ6 | rule step_load_byteI.succ2.succ7 |
+  rule step_load_byteI.succ2.word | rule step_load_byteI.succ2.true | rule step_load_byteI.succ2.false | 
+  rule step_load_byteI.succ2.storage |
+  rule step_load_byteI.succ2.unknown | rule step_load_byteI.succ2.xtract |
+  rule step_load_byteI.succ2.succ | rule step_load_byteI.succ2.succ2 | rule step_load_byteI.succ2.succ3 | 
+  rule step_load_byteI.succ2.succ4 | rule step_load_byteI.succ2.succ5 | rule step_load_byteI.succ2.succ6 | 
+  rule step_load_byteI.succ2.succ7 |
   rule step_load_byteI.succ2.val |
 
-  rule step_load_byteI.succ3.word | rule step_load_byteI.succ3.true | rule step_load_byteI.succ3.false | rule step_load_byteI.succ3.storage | rule step_load_byteI.succ3.unknown | rule step_load_byteI.succ3.xtract |
-  rule step_load_byteI.succ3.succ | rule step_load_byteI.succ3.succ2 | rule step_load_byteI.succ3.succ3 | rule step_load_byteI.succ3.succ4 | rule step_load_byteI.succ3.succ5 | rule step_load_byteI.succ3.succ6 | rule step_load_byteI.succ3.succ7 |
+  rule step_load_byteI.succ3.word | rule step_load_byteI.succ3.true | rule step_load_byteI.succ3.false | 
+  rule step_load_byteI.succ3.storage |
+  rule step_load_byteI.succ3.unknown | rule step_load_byteI.succ3.xtract |
+  rule step_load_byteI.succ3.succ | rule step_load_byteI.succ3.succ2 | rule step_load_byteI.succ3.succ3 | 
+  rule step_load_byteI.succ3.succ4 | rule step_load_byteI.succ3.succ5 | rule step_load_byteI.succ3.succ6 | 
+  rule step_load_byteI.succ3.succ7 |
   rule step_load_byteI.succ3.val |
 
-  rule step_load_byteI.succ4.word | rule step_load_byteI.succ4.true | rule step_load_byteI.succ4.false | rule step_load_byteI.succ4.storage | rule step_load_byteI.succ4.unknown | rule step_load_byteI.succ4.xtract |
-  rule step_load_byteI.succ4.succ | rule step_load_byteI.succ4.succ2 | rule step_load_byteI.succ4.succ3 | rule step_load_byteI.succ4.succ4 | rule step_load_byteI.succ4.succ5 | rule step_load_byteI.succ4.succ6 | rule step_load_byteI.succ4.succ7 |
+  rule step_load_byteI.succ4.word | rule step_load_byteI.succ4.true | rule step_load_byteI.succ4.false | 
+  rule step_load_byteI.succ4.storage |
+  rule step_load_byteI.succ4.unknown | rule step_load_byteI.succ4.xtract |
+  rule step_load_byteI.succ4.succ | rule step_load_byteI.succ4.succ2 | rule step_load_byteI.succ4.succ3 | 
+  rule step_load_byteI.succ4.succ4 | rule step_load_byteI.succ4.succ5 | rule step_load_byteI.succ4.succ6 | 
+  rule step_load_byteI.succ4.succ7 |
   rule step_load_byteI.succ4.val |
 
-  rule step_load_byteI.succ5.word | rule step_load_byteI.succ5.true | rule step_load_byteI.succ5.false | rule step_load_byteI.succ5.storage | rule step_load_byteI.succ5.unknown | rule step_load_byteI.succ5.xtract |
-  rule step_load_byteI.succ5.succ | rule step_load_byteI.succ5.succ2 | rule step_load_byteI.succ5.succ3 | rule step_load_byteI.succ5.succ4 | rule step_load_byteI.succ5.succ5 | rule step_load_byteI.succ5.succ6 | rule step_load_byteI.succ5.succ7 |
+  rule step_load_byteI.succ5.word | rule step_load_byteI.succ5.true | rule step_load_byteI.succ5.false | 
+  rule step_load_byteI.succ5.storage |
+  rule step_load_byteI.succ5.unknown | rule step_load_byteI.succ5.xtract |
+  rule step_load_byteI.succ5.succ | rule step_load_byteI.succ5.succ2 | rule step_load_byteI.succ5.succ3 | 
+  rule step_load_byteI.succ5.succ4 | rule step_load_byteI.succ5.succ5 | rule step_load_byteI.succ5.succ6 | rule step_load_byteI.succ5.succ7 |
   rule step_load_byteI.succ5.val |
 
-  rule step_load_byteI.succ6.word | rule step_load_byteI.succ6.true | rule step_load_byteI.succ6.false | rule step_load_byteI.succ6.storage | rule step_load_byteI.succ6.unknown | rule step_load_byteI.succ6.xtract |
-  rule step_load_byteI.succ6.succ | rule step_load_byteI.succ6.succ2 | rule step_load_byteI.succ6.succ3 | rule step_load_byteI.succ6.succ4 | rule step_load_byteI.succ6.succ5 | rule step_load_byteI.succ6.succ6 | rule step_load_byteI.succ6.succ7 |
+  rule step_load_byteI.succ6.word | rule step_load_byteI.succ6.true | rule step_load_byteI.succ6.false | 
+  rule step_load_byteI.succ6.storage |
+  rule step_load_byteI.succ6.unknown | rule step_load_byteI.succ6.xtract |
+  rule step_load_byteI.succ6.succ | rule step_load_byteI.succ6.succ2 | rule step_load_byteI.succ6.succ3 | 
+  rule step_load_byteI.succ6.succ4 | rule step_load_byteI.succ6.succ5 | rule step_load_byteI.succ6.succ6 | 
+  rule step_load_byteI.succ6.succ7 |
   rule step_load_byteI.succ6.val |
 
-  rule step_load_byteI.succ7.word | rule step_load_byteI.succ7.true | rule step_load_byteI.succ7.false | rule step_load_byteI.succ7.storage | rule step_load_byteI.succ7.unknown | rule step_load_byteI.succ7.xtract |
-  rule step_load_byteI.succ7.succ | rule step_load_byteI.succ7.succ2 | rule step_load_byteI.succ7.succ3 | rule step_load_byteI.succ7.succ4 | rule step_load_byteI.succ7.succ5 | rule step_load_byteI.succ7.succ6 | rule step_load_byteI.succ7.succ7 |
+  rule step_load_byteI.succ7.word | rule step_load_byteI.succ7.true | rule step_load_byteI.succ7.false | 
+  rule step_load_byteI.succ7.storage |
+  rule step_load_byteI.succ7.unknown | rule step_load_byteI.succ7.xtract |
+  rule step_load_byteI.succ7.succ | rule step_load_byteI.succ7.succ2 | rule step_load_byteI.succ7.succ3 | 
+  rule step_load_byteI.succ7.succ4 | rule step_load_byteI.succ7.succ5 | rule step_load_byteI.succ7.succ6 | rule step_load_byteI.succ7.succ7 |
   rule step_load_byteI.succ7.val |
-
-  step_load_byteI.intro_syntax |
 
   (rule step_load_byte_from_nextI.word.storage, solve_word_neq) |
   (rule step_load_byte_from_nextI.succ.storage, solve_word_neq) |
@@ -444,10 +382,18 @@ method solve_expI = (
   (rule step_load_byte_from_nextI.succ5.storage, solve_word_neq) |
   (rule step_load_byte_from_nextI.succ6.storage, solve_word_neq) |
   (rule step_load_byte_from_nextI.succ7.storage, solve_word_neq) |
+  (rule step_load_byte_from_nextI, solve_word_neq) |
 
-  (intro step_load_byte_from_nextI.syntaxs, linarith) | (* TODO *)
 
   (rule step_load_word_elI.storage.word, linarith) |
+  (rule step_load_word_elI.storage.succ, linarith) |
+  (rule step_load_word_elI.storage.succ2, linarith) |
+  (rule step_load_word_elI.storage.succ3, linarith) |
+  (rule step_load_word_elI.storage.succ4, linarith) |
+  (rule step_load_word_elI.storage.succ5, linarith) |
+  (rule step_load_word_elI.storage.succ6, linarith) |
+  (rule step_load_word_elI.storage.succ7, linarith) |
+  (rule step_load_word_elI.storage_addr.word, solve_typeI, linarith) |
   (rule step_load_word_elI.storage_addr.succ, solve_typeI, linarith) |
   (rule step_load_word_elI.storage_addr.succ2, solve_typeI, linarith) |
   (rule step_load_word_elI.storage_addr.succ3, solve_typeI, linarith) |
@@ -456,72 +402,94 @@ method solve_expI = (
   (rule step_load_word_elI.storage_addr.succ6, solve_typeI, linarith) |
   (rule step_load_word_elI.storage_addr.succ7, solve_typeI, linarith) |
 
+  (rule step_load_word_beI.storage.word, linarith) |
+  (rule step_load_word_beI.storage.succ, linarith) |
+  (rule step_load_word_beI.storage.succ2, linarith) |
+  (rule step_load_word_beI.storage.succ3, linarith) |
+  (rule step_load_word_beI.storage.succ4, linarith) |
+  (rule step_load_word_beI.storage.succ5, linarith) |
+  (rule step_load_word_beI.storage.succ6, linarith) |
+  (rule step_load_word_beI.storage.succ7, linarith) |
+  (rule step_load_word_beI.storage_addr.word, solve_typeI, linarith) |
+  (rule step_load_word_beI.storage_addr.succ, solve_typeI, linarith) |
+  (rule step_load_word_beI.storage_addr.succ2, solve_typeI, linarith) |
+  (rule step_load_word_beI.storage_addr.succ3, solve_typeI, linarith) |
+  (rule step_load_word_beI.storage_addr.succ4, solve_typeI, linarith) |
+  (rule step_load_word_beI.storage_addr.succ5, solve_typeI, linarith) |
+  (rule step_load_word_beI.storage_addr.succ6, solve_typeI, linarith) |
+  (rule step_load_word_beI.storage_addr.succ7, solve_typeI, linarith) |
 
-  (intro step_load_word_beI.syntaxs step_load_word_elI.syntaxs, linarith) |
-  (intro step_load_word_beI step_load_word_elI, linarith, solve_typeI) |
-  (rule step_load_memI.bv_plus, solve_expI) |
-  (intro step_load_memI.syntaxs, solve_expI) |
-  (rule step_load_addrI, solve_expI) |
+
+  (rule step_load_memI.bv_plus, solve_expI simp: simp) |
+  (rule step_load_addrI, solve_expI simp: simp) |
 
   \<comment> \<open>Store\<close>
-  (rule step_store_step_valI, solve_expI) |
-  (intro step_store_addrI.syntaxs, solve_expI) |
-  (intro step_store_memI.syntaxs2, solve_expI) |
-  (intro step_store_un_addrI.syntaxs2, solve_typeI) |
-  (intro step_store_valI.val.syntaxs, solve_typeI) |
-  (intro step_store_word_elI.storage.syntaxs step_store_word_elI.unknown.syntaxs step_store_word_beI.storage.syntaxs step_store_word_beI.unknown.syntaxs, linarith, blast) |
-  (intro step_store_word_elI.val.syntaxs step_store_word_beI.val.syntaxs, solve_typeI, linarith, blast) |
+  (rule step_store_valI.word.storage.xtract) |
+  (rule step_store_valI.word.storage_addr.xtract, solve_typeI) |
+  (rule step_store_valI.word.val.xtract, solve_typeI) |
+  (rule step_store_valI.succ.storage.xtract) |
+  (rule step_store_valI.succ.storage_addr.xtract, solve_typeI) |
+  (rule step_store_valI.succ.val.xtract, solve_typeI) |
+  (rule step_store_valI.succ2.storage.xtract) |
+  (rule step_store_valI.succ2.storage_addr.xtract, solve_typeI) |
+  (rule step_store_valI.succ2.val.xtract, solve_typeI) |
+  (rule step_store_valI.succ3.storage.xtract) |
+  (rule step_store_valI.succ3.storage_addr.xtract, solve_typeI) |
+  (rule step_store_valI.succ3.val.xtract, solve_typeI) |
+  (rule step_store_valI.succ4.storage.xtract) |
+  (rule step_store_valI.succ4.storage_addr.xtract, solve_typeI) |
+  (rule step_store_valI.succ4.val.xtract, solve_typeI) |
+  (rule step_store_valI.succ5.storage.xtract) |
+  (rule step_store_valI.succ5.storage_addr.xtract, solve_typeI) |
+  (rule step_store_valI.succ5.val.xtract, solve_typeI) |
+  (rule step_store_valI.succ6.storage.xtract) |
+  (rule step_store_valI.succ6.storage_addr.xtract, solve_typeI) |
+  (rule step_store_valI.succ6.val.xtract, solve_typeI) |
+  (rule step_store_valI.succ7.storage.xtract) |
+  (rule step_store_valI.succ7.storage_addr.xtract, solve_typeI) |
+  (rule step_store_valI.succ7.val.xtract, solve_typeI) |
+
+  (rule step_store_step_valI, solve_expI simp: simp) |
 
   \<comment> \<open>Let\<close>
-  (rule step_let_stepI, solve_expI) |
+  (rule step_let_stepI, solve_expI simp: simp) |
 
   \<comment> \<open>Ite\<close>
-  (rule step_ite_elseI, solve_expI) |
-  (intro step_ite_condI.syntaxs2, solve_expI) |
-  (intro step_ite_thenI.syntaxs, solve_expI) |
-  (intro step_ite_unI.syntaxs2, solve_typeI) |
+  (rule step_ite_elseI, solve_expI simp: simp) |
 
   \<comment> \<open>Bop\<close>
-  (intro step_plusI.lhsI step_minusI.lhsI step_timesI.lhsI step_divideI.lhsI step_sdivideI.lhsI 
-   step_modI.lhsI step_smodI.lhsI step_lslI.lhsI step_lsrI.lhsI step_asrI.lhsI step_landI.lhsI 
-   step_lorI.lhsI step_xorI.lhsI step_ltI.lhsI step_leI.lhsI step_sltI.lhsI step_sleI.lhsI, solve_expI) |
-  (intro step_plusI.rhs.syntaxs step_minusI.rhs.syntaxs step_timesI.rhs.syntaxs step_divideI.rhs.syntaxs 
-   step_sdivideI.rhs.syntaxs step_modI.rhs.syntaxs step_smodI.rhs.syntaxs step_lslI.rhs.syntaxs 
-   step_lsrI.rhs.syntaxs step_asrI.rhs.syntaxs step_landI.rhs.syntaxs step_lorI.rhs.syntaxs 
-   step_xorI.rhs.syntaxs step_leI.rhs.syntaxs step_ltI.rhs.syntaxs step_sleI.rhs.syntaxs 
-   step_sltI.rhs.syntaxs, solve_expI) |
 
   \<comment> \<open>Plus\<close>
   (rule step_plusI) |
-  (rule step_plusI.lhsI, solve_expI) |
+  (rule step_plusI.lhsI, solve_expI simp: simp) |
  
   \<comment> \<open>Uop\<close>
   rule step_not_trueI | rule step_not_falseI | rule step_uop_unk_notI | rule step_uop_unk_negI |
   rule step_uop_unkI  | rule step_notI       | rule step_negI         |
-  (rule step_uopI, solve_expI) |
+  (rule step_uopI, solve_expI simp: simp) |
 
   \<comment> \<open>Concat\<close>
   rule step_concatI | rule step_concatI.xtract.xtract |
 
-  (rule step_concat_lhsI.word, solve_expI) | 
-  (rule step_concat_lhsI.xtract, solve_expI) |
+  (rule step_concat_lhsI.word, solve_expI simp: simp) | 
+  (rule step_concat_lhsI.xtract, solve_expI simp: simp) |
 
-  (rule step_concat_rhsI, solve_expI) |
+  (rule step_concat_rhsI, solve_expI simp: simp) |
   (rule step_concat_lhs_unI, solve_typeI) |
   (rule step_concat_rhs_unI, solve_typeI) |
 
   \<comment> \<open>Extract\<close>
   rule step_extractI | rule step_extract_unI | 
-  (rule step_extract_reduceI, solve_expI) |
+  (rule step_extract_reduceI, solve_expI simp: simp) |
 
   \<comment> \<open>Cast\<close>
-  (rule step_cast_lowI) | 
-  (rule step_cast_highI) | 
-  (rule step_cast_signedI) | 
-  (rule step_cast_unsignedI) | 
+  (rule step_cast_lowI) |  (rule step_cast_lowI.xtract) |
+  (rule step_cast_highI) | (rule step_cast_highI.xtract) |
+  (rule step_cast_signedI) | (rule step_cast_signedI.xtract) |
+  (rule step_cast_unsignedI) | (rule step_cast_unsignedI.xtract) |
   (rule step_cast_unkI) | 
-  (rule step_cast_reduceI, solve_expI)
-)
+  (rule step_cast_reduceI, solve_expI simp: simp)
+))
 
 text \<open>Match names of the rules from the manual\<close>
 
