ExpressionSemantics/Expressions_Rules.thy
@@ -25,50 +25,68 @@ context storage_constructor
 begin
 
 abbreviation 
-  storage16 :: \<open>val \<Rightarrow> nat \<Rightarrow> nat \<Rightarrow> nat \<Rightarrow> 'a\<close>
+  storage16 :: \<open>val \<Rightarrow> word \<Rightarrow> val \<Rightarrow> 'a\<close>
 where
-  \<open>storage16 mem num\<^sub>1 sz\<^sub>a\<^sub>d\<^sub>d\<^sub>r num\<^sub>2 \<equiv> (mem
-    [num\<^sub>1 \<Colon> sz\<^sub>a\<^sub>d\<^sub>d\<^sub>r \<leftarrow> ext num\<^sub>2 \<Colon> 16 \<sim> hi :  7 \<sim> lo :  0, 8]
-    [succ (num\<^sub>1 \<Colon> sz\<^sub>a\<^sub>d\<^sub>d\<^sub>r) \<leftarrow> ext num\<^sub>2 \<Colon> 16 \<sim> hi : 15 \<sim> lo :  8, 8])
+  \<open>storage16 mem w v \<equiv> (mem
+    [w \<leftarrow> ext v \<sim> hi :  7 \<sim> lo :  0, 8]
+    [succ w \<leftarrow> ext v \<sim> hi : 15 \<sim> lo :  8, 8])
 \<close>
 
 abbreviation (* TODO addresses *)
-  storage32 :: \<open>val \<Rightarrow> nat \<Rightarrow> nat \<Rightarrow> nat \<Rightarrow> 'a\<close>
+  storage32 :: \<open>val \<Rightarrow> word \<Rightarrow> val \<Rightarrow> 'a\<close>
 where
-  \<open>storage32 mem num\<^sub>1 sz\<^sub>a\<^sub>d\<^sub>d\<^sub>r num\<^sub>2 \<equiv> (mem
-    [num\<^sub>1 \<Colon> sz\<^sub>a\<^sub>d\<^sub>d\<^sub>r \<leftarrow> ext num\<^sub>2 \<Colon> 32 \<sim> hi :  7 \<sim> lo :  0, 8]
-    [succ (num\<^sub>1 \<Colon> sz\<^sub>a\<^sub>d\<^sub>d\<^sub>r) \<leftarrow> ext num\<^sub>2 \<Colon> 32 \<sim> hi : 15 \<sim> lo :  8, 8]
-    [succ (succ (num\<^sub>1 \<Colon> sz\<^sub>a\<^sub>d\<^sub>d\<^sub>r)) \<leftarrow> ext num\<^sub>2 \<Colon> 32 \<sim> hi : 23 \<sim> lo : 16, 8]
-    [succ (succ (succ (num\<^sub>1 \<Colon> sz\<^sub>a\<^sub>d\<^sub>d\<^sub>r))) \<leftarrow> ext num\<^sub>2 \<Colon> 32 \<sim> hi : 31 \<sim> lo : 24, 8])
+  \<open>storage32 mem w v \<equiv> (mem
+    [w \<leftarrow> ext v \<sim> hi :  7 \<sim> lo :  0, 8]
+    [succ w \<leftarrow> ext v \<sim> hi : 15 \<sim> lo :  8, 8]
+    [succ (succ w) \<leftarrow> ext v \<sim> hi : 23 \<sim> lo : 16, 8]
+    [succ (succ (succ w)) \<leftarrow> ext v \<sim> hi : 31 \<sim> lo : 24, 8])
 \<close>
 
 abbreviation 
-  storage64 :: \<open>val \<Rightarrow> nat \<Rightarrow> nat \<Rightarrow> nat \<Rightarrow> 'a\<close>
+  storage_el64 :: \<open>val \<Rightarrow> word \<Rightarrow> val \<Rightarrow> 'a\<close>
 where
-  \<open>storage64 mem num\<^sub>1 sz\<^sub>a\<^sub>d\<^sub>d\<^sub>r num\<^sub>2 \<equiv> (mem
-    [num\<^sub>1 \<Colon> sz\<^sub>a\<^sub>d\<^sub>d\<^sub>r \<leftarrow> ext num\<^sub>2 \<Colon> 64 \<sim> hi :  7 \<sim> lo :  0, 8]
-    [succ (num\<^sub>1 \<Colon> sz\<^sub>a\<^sub>d\<^sub>d\<^sub>r) \<leftarrow> ext num\<^sub>2 \<Colon> 64 \<sim> hi : 15 \<sim> lo :  8, 8]
-    [succ (succ (num\<^sub>1 \<Colon> sz\<^sub>a\<^sub>d\<^sub>d\<^sub>r)) \<leftarrow> ext num\<^sub>2 \<Colon> 64 \<sim> hi : 23 \<sim> lo : 16, 8]
-    [succ (succ (succ (num\<^sub>1 \<Colon> sz\<^sub>a\<^sub>d\<^sub>d\<^sub>r))) \<leftarrow> ext num\<^sub>2 \<Colon> 64 \<sim> hi : 31 \<sim> lo : 24, 8]
-    [succ (succ (succ (succ (num\<^sub>1 \<Colon> sz\<^sub>a\<^sub>d\<^sub>d\<^sub>r)))) \<leftarrow> ext num\<^sub>2 \<Colon> 64 \<sim> hi : 39 \<sim> lo : 32, 8]
-    [succ (succ (succ (succ (succ (num\<^sub>1 \<Colon> sz\<^sub>a\<^sub>d\<^sub>d\<^sub>r))))) \<leftarrow> ext num\<^sub>2 \<Colon> 64 \<sim> hi : 47 \<sim> lo : 40, 8]
-    [succ (succ (succ (succ (succ (succ (num\<^sub>1 \<Colon> sz\<^sub>a\<^sub>d\<^sub>d\<^sub>r)))))) \<leftarrow> ext num\<^sub>2 \<Colon> 64 \<sim> hi : 55 \<sim> lo : 48, 8]
-    [succ (succ (succ (succ (succ (succ (succ (num\<^sub>1 \<Colon> sz\<^sub>a\<^sub>d\<^sub>d\<^sub>r))))))) \<leftarrow> ext num\<^sub>2 \<Colon> 64 \<sim> hi : 63 \<sim> lo : 56, 8])
+  \<open>storage_el64 mem w v \<equiv> (mem
+    [w \<leftarrow> ext v \<sim> hi :  7 \<sim> lo :  0, 8]
+    [succ w \<leftarrow> ext v \<sim> hi : 15 \<sim> lo :  8, 8]
+    [succ (succ w) \<leftarrow> ext v \<sim> hi : 23 \<sim> lo : 16, 8]
+    [succ (succ (succ w)) \<leftarrow> ext v \<sim> hi : 31 \<sim> lo : 24, 8]
+    [succ (succ (succ (succ w))) \<leftarrow> ext v \<sim> hi : 39 \<sim> lo : 32, 8]
+    [succ (succ (succ (succ (succ w)))) \<leftarrow> ext v \<sim> hi : 47 \<sim> lo : 40, 8]
+    [succ (succ (succ (succ (succ (succ w))))) \<leftarrow> ext v \<sim> hi : 55 \<sim> lo : 48, 8]
+    [succ (succ (succ (succ (succ (succ (succ w)))))) \<leftarrow> ext v \<sim> hi : 63 \<sim> lo : 56, 8])
+\<close>
+
+abbreviation 
+  storage_be64 :: \<open>val \<Rightarrow> word \<Rightarrow> val \<Rightarrow> 'a\<close>
+where
+  \<open>storage_be64 mem w v \<equiv> (mem
+    [w \<leftarrow> ext v \<sim> hi : 63 \<sim> lo :  56, 8]
+    [succ w \<leftarrow> ext v \<sim> hi : 55 \<sim> lo : 48, 8]
+    [succ (succ w) \<leftarrow> ext v \<sim> hi : 47 \<sim> lo : 40, 8]
+    [succ (succ (succ w)) \<leftarrow> ext v \<sim> hi : 39 \<sim> lo : 32, 8]
+    [succ (succ (succ (succ w))) \<leftarrow> ext v \<sim> hi : 31 \<sim> lo : 24, 8]
+    [succ (succ (succ (succ (succ w)))) \<leftarrow> ext v \<sim> hi : 23 \<sim> lo : 16, 8]
+    [succ (succ (succ (succ (succ (succ w))))) \<leftarrow> ext v \<sim> hi : 15 \<sim> lo : 8, 8]
+    [succ (succ (succ (succ (succ (succ (succ w)))))) \<leftarrow> ext v \<sim> hi : 7 \<sim> lo : 0, 8])
 \<close>
 
 end
 
-lemma type_storage16: \<open>type (storage16 mem address sz\<^sub>a\<^sub>d\<^sub>d\<^sub>r val\<^sub>1) = mem\<langle>sz\<^sub>a\<^sub>d\<^sub>d\<^sub>r, 8\<rangle>\<close>
+lemma type_storage16: \<open>type (storage16 mem (num \<Colon> sz\<^sub>a\<^sub>d\<^sub>d\<^sub>r) val\<^sub>1) = mem\<langle>sz\<^sub>a\<^sub>d\<^sub>d\<^sub>r, 8\<rangle>\<close>
   unfolding succ.simps bv_plus.simps by (rule type_storageI)
 
-lemma type_storage32: \<open>type (storage32 mem address sz\<^sub>a\<^sub>d\<^sub>d\<^sub>r val\<^sub>1) = mem\<langle>sz\<^sub>a\<^sub>d\<^sub>d\<^sub>r, 8\<rangle>\<close>
+lemma type_storage32: \<open>type (storage32 mem (num \<Colon> sz\<^sub>a\<^sub>d\<^sub>d\<^sub>r) val\<^sub>1) = mem\<langle>sz\<^sub>a\<^sub>d\<^sub>d\<^sub>r, 8\<rangle>\<close>
   unfolding succ.simps bv_plus.simps by (rule type_storageI)
 
-lemma type_storage64: \<open>type (storage64 mem address sz\<^sub>a\<^sub>d\<^sub>d\<^sub>r val\<^sub>1) = mem\<langle>sz\<^sub>a\<^sub>d\<^sub>d\<^sub>r, 8\<rangle>\<close>
+lemma type_storage_el64: \<open>type (storage_el64 mem (num \<Colon> sz\<^sub>a\<^sub>d\<^sub>d\<^sub>r) val\<^sub>1) = mem\<langle>sz\<^sub>a\<^sub>d\<^sub>d\<^sub>r, 8\<rangle>\<close>
+  unfolding succ.simps bv_plus.simps by (rule type_storageI)
+
+lemma type_storage_be64: \<open>type (storage_be64 mem (num \<Colon> sz\<^sub>a\<^sub>d\<^sub>d\<^sub>r) val\<^sub>1) = mem\<langle>sz\<^sub>a\<^sub>d\<^sub>d\<^sub>r, 8\<rangle>\<close>
   unfolding succ.simps bv_plus.simps by (rule type_storageI)
 
 method solve_type_storage = (
-    rule type_storage64 | rule type_storage32 | rule type_storage16 | rule type_storageI
+    rule type_storage_el64 | rule type_storage32 | rule type_storage16 | rule type_storageI |
+    rule type_storage_be64 | rule type_storage32 | rule type_storage16 | rule type_storageI
 )
 
 end
