Parser/Lexer.thy
@@ -17,16 +17,16 @@ where
       bargstr = dropWhile isnt_lbracket tstr;
       argstr = butlast (tl bargstr)
     in
-      Node name (map lexer (split argstr))
+      Node name (map lexer (split_not_within argstr))
   )\<close>
   by auto
 termination apply standard
   apply (rule wf_mlex[of \<open>{}\<close> length])
-  apply (auto simp del: split.simps)
+  apply (auto simp del: split_not_within.simps)
   apply (rule mlex_less)
   subgoal for str xd
     apply (cases str, simp)
-    apply (drule length_split, auto)
+    apply (drule length_split_not_within, auto)
     by (smt (verit, ccfv_SIG) One_nat_def diff_Suc_eq_diff_pred diff_is_0_eq' diff_less leD leI le_trans length_append_singleton length_dropWhile_le length_rev linordered_nonzero_semiring_class.zero_le_one zero_less_Suc)
   .
 
