Prelims/AST_Prelims.thy
@@ -2,7 +2,12 @@ theory AST_Prelims
   imports Result
 begin
 
-abbreviation \<open>is_whitespace x \<equiv> (x = CHR '' '' \<or> x = CHR 0x9 \<or> x = CHR 10 \<or> x = CHR 13)\<close>
+abbreviation \<open>TAB \<equiv> CHR 9\<close>
+abbreviation \<open>VT \<equiv> CHR 11\<close>
+abbreviation \<open>CR \<equiv> CHR 13\<close>
+abbreviation \<open>LF \<equiv> CHR 10\<close>
+
+abbreviation \<open>is_whitespace x \<equiv> (x = CHR '' '' \<or> x = TAB \<or> x = LF \<or> x = VT \<or> x = CR)\<close>
 
 definition
   triml :: \<open>string \<Rightarrow> string\<close>
@@ -41,12 +46,6 @@ lemma trim_empty[simp]: \<open>trim '''' = ''''\<close>
 lemma ascii_of_ascii_of[simp]: \<open>String.ascii_of (String.ascii_of x) = String.ascii_of x\<close>
   using String.ascii_of_idem by auto
 
-
-
-
-datatype AST = Node string \<open>AST list\<close>
-
-
 fun 
   insert_hd :: \<open>'a \<Rightarrow> 'a list list \<Rightarrow> 'a list list\<close>
 where
@@ -56,15 +55,50 @@ where
 lemma length_insert_hd: \<open>length xs \<le> length (insert_hd x xs)\<close>
   by (induct xs, auto)
 
+
 function
-  split_string :: \<open>string \<Rightarrow> nat \<Rightarrow> string list\<close>
+  split :: \<open>'a \<Rightarrow> 'a list \<Rightarrow> 'a list list\<close>
 where
-  \<open>split_string [] _ = []\<close> |
-  \<open>split_string (CHR '','' # cs) 0 = [] # split_string cs 0\<close> |
-  \<open>split_string (CHR ''('' # cs) ctr = insert_hd (CHR ''('') (split_string cs (ctr + 1))\<close> |
-  \<open>split_string (CHR '')'' # cs) ctr = insert_hd (CHR '')'') (split_string cs (ctr - 1))\<close> |
+  \<open>split _ [] = []\<close> |
+  \<open>split c (c # str) = [] # split c str\<close> |
+  \<open>\<lbrakk>c' \<noteq> c\<rbrakk> \<Longrightarrow> split c (c' # str) = (insert_hd c' (split c str))\<close>
+  subgoal for _ x
+    apply (cases x, auto)
+    subgoal for c str
+      by (cases str, auto)
+    .
+  by auto
+termination by lexicographic_order
+
+declare split.simps(2)[simp del]
+
+lemma split_eq_char[simp]: \<open>split c (c # str) = [] # split c str\<close>
+  unfolding split.simps by simp
+
+lemma split_neq_char[simp]: 
+  assumes \<open>c' \<noteq> c\<close>
+    shows \<open>split c (c' # str) = insert_hd c' (split c str)\<close>
+  using assms unfolding split.simps by auto
+
+lemma [code]: 
+  \<open>split c [] = []\<close>
+  \<open>split c (c' # str) = (if (c = c') then [] # split c str else insert_hd c' (split c str))\<close>
+  by auto
+
+
+datatype AST = Node string \<open>AST list\<close>
+
+
+
+function
+  split_not_within_int :: \<open>string \<Rightarrow> nat \<Rightarrow> string list\<close>
+where
+  \<open>split_not_within_int [] _ = []\<close> |
+  \<open>split_not_within_int (CHR '','' # cs) 0 = [] # split_not_within_int cs 0\<close> |
+  \<open>split_not_within_int (CHR ''('' # cs) ctr = insert_hd (CHR ''('') (split_not_within_int cs (ctr + 1))\<close> |
+  \<open>split_not_within_int (CHR '')'' # cs) ctr = insert_hd (CHR '')'') (split_not_within_int cs (ctr - 1))\<close> |
   \<open>\<lbrakk>c \<noteq> CHR ''(''; c \<noteq> CHR '')''; ctr = 0 \<longrightarrow> c \<noteq> CHR '',''\<rbrakk> \<Longrightarrow> 
-    split_string (c # cs) ctr = insert_hd c (split_string cs ctr)\<close>
+    split_not_within_int (c # cs) ctr = insert_hd c (split_not_within_int cs ctr)\<close>
   subgoal for _ x apply (cases x, auto)
     subgoal for x y by (cases x, auto)
     .
@@ -72,26 +106,26 @@ where
 termination by lexicographic_order
 
 lemma [code]: 
-  \<open>split_string [] ctr = []\<close>
-\<open>split_string (c # str) ctr = (
-  if (c = CHR '','' \<and> ctr = 0) then [] # split_string str 0
-  else if (c = CHR ''('') then insert_hd (CHR ''('') (split_string str (ctr + 1))
-  else if (c = CHR '')'') then insert_hd (CHR '')'') (split_string str (ctr - 1))
-  else insert_hd c (split_string str ctr))\<close>
+  \<open>split_not_within_int [] ctr = []\<close>
+\<open>split_not_within_int (c # str) ctr = (
+  if (c = CHR '','' \<and> ctr = 0) then [] # split_not_within_int str 0
+  else if (c = CHR ''('') then insert_hd (CHR ''('') (split_not_within_int str (ctr + 1))
+  else if (c = CHR '')'') then insert_hd (CHR '')'') (split_not_within_int str (ctr - 1))
+  else insert_hd c (split_not_within_int str ctr))\<close>
   by (auto split: if_split)
 
 fun
-  split :: \<open>string \<Rightarrow> string list\<close>
+  split_not_within :: \<open>string \<Rightarrow> string list\<close>
 where
-  \<open>split s = split_string s 0\<close>
+  \<open>split_not_within s = split_not_within_int s 0\<close>
 
-lemma split_empty[simp]: \<open>split [] = []\<close>
+lemma split_empty[simp]: \<open>split_not_within [] = []\<close>
   by auto
 
-lemma length_split:
-  assumes \<open>xd \<in> set (split xs)\<close>
+lemma length_split_not_within:
+  assumes \<open>xd \<in> set (split_not_within xs)\<close>
     shows \<open>length xd \<le> length xs\<close>
-using assms unfolding split.simps proof (induction arbitrary: xd rule: split_string.induct[of _ xs 0])
+using assms unfolding split_not_within.simps proof (induction arbitrary: xd rule: split_not_within_int.induct[of _ xs 0])
   case (2 cs)
   then show ?case 
     apply auto    
@@ -100,21 +134,21 @@ next
   case (3 cs ctr)
   then show ?case 
     apply auto
-    apply (cases \<open>split_string cs (Suc ctr)\<close>, auto)
+    apply (cases \<open>split_not_within_int cs (Suc ctr)\<close>, auto)
     using le_SucI by presburger
 next
   case (4 cs ctr)
   then show ?case 
     apply auto
-    apply (cases \<open>split_string cs (ctr - Suc 0)\<close>, auto)
+    apply (cases \<open>split_not_within_int cs (ctr - Suc 0)\<close>, auto)
     using le_SucI by presburger
 next
   case (5 c ctr cs)
   then show ?case
     apply auto
-    apply (cases \<open>split_string cs ctr\<close>, auto)
+    apply (cases \<open>split_not_within_int cs ctr\<close>, auto)
     using le_SucI apply presburger
-    apply (cases \<open>split_string cs ctr\<close>, auto)
+    apply (cases \<open>split_not_within_int cs ctr\<close>, auto)
     using le_SucI by presburger
 qed auto
 
@@ -123,51 +157,93 @@ type_synonym 'v parser_result = \<open>('v, string) result\<close>
 
 abbreviation \<open>ord0 \<equiv> of_char (CHR ''0'')\<close>
 abbreviation \<open>ord9 \<equiv> of_char (CHR ''9'')\<close>
+abbreviation \<open>orda \<equiv> of_char (CHR ''a'')\<close>
+abbreviation \<open>ordA \<equiv> of_char (CHR ''A'')\<close>
+abbreviation \<open>ordz \<equiv> of_char (CHR ''z'')\<close>
+abbreviation \<open>ordZ \<equiv> of_char (CHR ''Z'')\<close>
 
-text \<open>Converts a char ordinal to a numeric type\<close>
+
+
+text \<open>Converts a char ordinal to a numeric type (with radix)\<close>
 
 definition
-  of_char_ord :: \<open>char \<Rightarrow> ('a::{minus,ord,comm_semiring_1}) parser_result\<close>
+  of_char_radix :: \<open>('a::{minus,ord,comm_semiring_1}) \<Rightarrow> char \<Rightarrow>  ('a::{minus,ord,comm_semiring_1}) parser_result\<close>
 where
-  \<open>of_char_ord c = (
+  \<open>of_char_radix radix c  = (
     let 
       ord = of_char c 
     in
-      if (ord < ord0 \<or> ord > ord9)
-      then Error (List.append ''Codepoint out of range (48-57): '' [c])
-      else Value (ord - ord0)
+      if (radix > 36) then Error (List.append ''Radix out of range (>36): '' [c])
+      else if (ord0 \<le> ord \<and> ord \<le> max ord9 radix) then Value (ord - ord0)
+      else if (radix > 10 \<and> orda \<le> ord \<and> ord \<le> orda + (radix - 11)) then Value (ord - orda + 10)
+      else if (radix > 10 \<and> ordA \<le> ord \<and> ord \<le> ordA + (radix - 11)) then Value (ord - ordA + 10)
+      else Error (List.append ''Codepoint out of range for radix: '' [c])
   )\<close>
 
-lemma of_char_ord_linordered_semidom[simp]: \<open>of_char_ord (CHR ''0'') = Value (0::'a::linordered_semidom)\<close>
-  unfolding of_char_ord_def by auto
+abbreviation
+  of_char_dec :: \<open>char \<Rightarrow> ('a::{minus,ord,comm_semiring_1}) parser_result\<close>
+where
+  \<open>of_char_dec \<equiv> of_char_radix 10\<close>
 
-lemma of_char_ord_nat[simp]:
-  \<open>of_char_ord (CHR ''1'') = Value (1::nat)\<close> \<open>of_char_ord (CHR ''2'') = Value (2::nat)\<close>
-  \<open>of_char_ord (CHR ''3'') = Value (3::nat)\<close> \<open>of_char_ord (CHR ''4'') = Value (4::nat)\<close>
-  \<open>of_char_ord (CHR ''5'') = Value (5::nat)\<close> \<open>of_char_ord (CHR ''6'') = Value (6::nat)\<close>
-  \<open>of_char_ord (CHR ''7'') = Value (7::nat)\<close> \<open>of_char_ord (CHR ''8'') = Value (8::nat)\<close>
-  \<open>of_char_ord (CHR ''9'') = Value (9::nat)\<close>
-  unfolding of_char_ord_def by auto
+lemma of_char_dec_linordered_semidom[simp]: \<open>of_char_dec (CHR ''0'') = Value (0::'a::linordered_semidom)\<close>
+  unfolding of_char_radix_def by auto
+
+lemma of_char_dec_nat[simp]:
+  \<open>of_char_dec (CHR ''1'') = Value (1::nat)\<close> \<open>of_char_dec (CHR ''2'') = Value (2::nat)\<close>
+  \<open>of_char_dec (CHR ''3'') = Value (3::nat)\<close> \<open>of_char_dec (CHR ''4'') = Value (4::nat)\<close>
+  \<open>of_char_dec (CHR ''5'') = Value (5::nat)\<close> \<open>of_char_dec (CHR ''6'') = Value (6::nat)\<close>
+  \<open>of_char_dec (CHR ''7'') = Value (7::nat)\<close> \<open>of_char_dec (CHR ''8'') = Value (8::nat)\<close>
+  \<open>of_char_dec (CHR ''9'') = Value (9::nat)\<close>
+  unfolding of_char_radix_def by auto
   
-lemma of_char_ord_0_9: \<open>of_char_ord c = Value v \<Longrightarrow> (v::nat) \<in> {0..9}\<close>
-  unfolding of_char_ord_def Let_def by (auto split: if_splits)
+lemma of_char_dec_0_9: \<open>of_char_dec c = Value v \<Longrightarrow> (v::nat) \<in> {0..9}\<close>
+  unfolding of_char_radix_def Let_def by (auto split: if_splits)
+
+abbreviation
+  of_char_hex :: \<open>char \<Rightarrow> ('a::{minus,ord,comm_semiring_1}) parser_result\<close>
+where
+  \<open>of_char_hex \<equiv> of_char_radix 16\<close>
+
+lemma of_char_hex_linordered_semidom[simp]: \<open>of_char_hex (CHR ''0'') = Value (0::'a::linordered_semidom)\<close>
+  unfolding of_char_radix_def by auto
+
+lemma of_char_hex_nat[simp]:
+  \<open>of_char_hex (CHR ''1'') = Value (1::nat)\<close> \<open>of_char_hex (CHR ''2'') = Value (2::nat)\<close>
+  \<open>of_char_hex (CHR ''3'') = Value (3::nat)\<close> \<open>of_char_hex (CHR ''4'') = Value (4::nat)\<close>
+  \<open>of_char_hex (CHR ''5'') = Value (5::nat)\<close> \<open>of_char_hex (CHR ''6'') = Value (6::nat)\<close>
+  \<open>of_char_hex (CHR ''7'') = Value (7::nat)\<close> \<open>of_char_hex (CHR ''8'') = Value (8::nat)\<close>
+  \<open>of_char_hex (CHR ''9'') = Value (9::nat)\<close>
+  \<open>of_char_hex (CHR ''a'') = Value (10::nat)\<close> \<open>of_char_hex (CHR ''A'') = Value (10::nat)\<close>
+  \<open>of_char_hex (CHR ''b'') = Value (11::nat)\<close> \<open>of_char_hex (CHR ''B'') = Value (11::nat)\<close>
+  \<open>of_char_hex (CHR ''c'') = Value (12::nat)\<close> \<open>of_char_hex (CHR ''C'') = Value (12::nat)\<close>
+  \<open>of_char_hex (CHR ''d'') = Value (13::nat)\<close> \<open>of_char_hex (CHR ''D'') = Value (13::nat)\<close>
+  \<open>of_char_hex (CHR ''e'') = Value (14::nat)\<close> \<open>of_char_hex (CHR ''E'') = Value (14::nat)\<close>
+  \<open>of_char_hex (CHR ''f'') = Value (15::nat)\<close> \<open>of_char_hex (CHR ''F'') = Value (15::nat)\<close>
+  unfolding of_char_radix_def Let_def by auto
+  
+lemma of_char_hex_0_16: \<open>of_char_hex c = Value v \<Longrightarrow> (v::nat) \<in> {0..15}\<close>
+  unfolding of_char_radix_def Let_def by (auto split: if_splits)
+
 
 fun
-  nat_of_string  :: \<open>string \<Rightarrow> nat parser_result\<close>
+  nat_of_string_radix  :: \<open>nat \<Rightarrow> string \<Rightarrow> nat parser_result\<close>
 where
-  \<open>nat_of_string [] = Error ''Cannot convert empty string to nat''\<close> |
-  \<open>nat_of_string [c] = of_char_ord c\<close> |
-  \<open>nat_of_string (c # str) = (
-    Result.bind (of_char_ord c) (\<lambda>d. map_result_value (\<lambda>m. 10 * d + m) (nat_of_string str))
+  \<open>nat_of_string_radix _ [] = Error ''Cannot convert empty string to nat''\<close> |
+  \<open>nat_of_string_radix radix [c] = of_char_radix radix c\<close> |
+  \<open>nat_of_string_radix radix (c # str) = (
+    Result.bind (of_char_radix radix c) (\<lambda>d. map_result_value (\<lambda>m. (radix ^ length str) * d + m) (nat_of_string_radix radix str))
   )\<close>
+
+abbreviation \<open>nat_of_dec_string \<equiv> nat_of_string_radix 10\<close>
+abbreviation \<open>nat_of_hex_string \<equiv> nat_of_string_radix 16\<close>
 
 fun
   int_of_string  :: \<open>string \<Rightarrow> int parser_result\<close>
 where
   \<open>int_of_string [] = Error ''Cannot convert empty string to int''\<close> |
   \<open>int_of_string (c # str) = (
-    if c = CHR ''-'' then map_result_value (\<lambda>x. x * -1) (map_result_value of_nat (nat_of_string str))
-    else map_result_value of_nat (nat_of_string (c # str))
+    if c = CHR ''-'' then map_result_value (\<lambda>x. x * -1) (map_result_value of_nat (nat_of_dec_string str))
+    else map_result_value of_nat (nat_of_dec_string (c # str))
   )\<close>
 
 
