extras/Mem64_Intros.thy
@@ -6,71 +6,6 @@ begin
 
 text \<open>Memory extension\<close>
 
-(* TODO *)
-lemma step_concat_extractI: \<open>\<Delta> \<turnstile> ((ext num\<^sub>1 \<Colon> sz\<^sub>1 \<sim> hi : sz\<^sub>h\<^sub>i\<^sub>1 \<sim> lo : sz\<^sub>l\<^sub>o\<^sub>1) @ ext num\<^sub>2 \<Colon> sz\<^sub>2 \<sim> hi : sz\<^sub>h\<^sub>i\<^sub>2 \<sim> lo : sz\<^sub>l\<^sub>o\<^sub>2) \<leadsto> ((ext num\<^sub>1 \<Colon> sz\<^sub>1 \<sim> hi : sz\<^sub>h\<^sub>i\<^sub>1 \<sim> lo : sz\<^sub>l\<^sub>o\<^sub>1) \<cdot> ext num\<^sub>2 \<Colon> sz\<^sub>2 \<sim> hi : sz\<^sub>h\<^sub>i\<^sub>2 \<sim> lo : sz\<^sub>l\<^sub>o\<^sub>2)\<close>
-  unfolding xtract.simps by (rule step_concatI)
-
-lemma step_exps_concat_extractI: \<open>\<Delta> \<turnstile> ((ext num\<^sub>1 \<Colon> sz\<^sub>1 \<sim> hi : sz\<^sub>h\<^sub>i\<^sub>1 \<sim> lo : sz\<^sub>l\<^sub>o\<^sub>1) @ ext num\<^sub>2 \<Colon> sz\<^sub>2 \<sim> hi : sz\<^sub>h\<^sub>i\<^sub>2 \<sim> lo : sz\<^sub>l\<^sub>o\<^sub>2) \<leadsto>* ((ext num\<^sub>1 \<Colon> sz\<^sub>1 \<sim> hi : sz\<^sub>h\<^sub>i\<^sub>1 \<sim> lo : sz\<^sub>l\<^sub>o\<^sub>1) \<cdot> ext num\<^sub>2 \<Colon> sz\<^sub>2 \<sim> hi : sz\<^sub>h\<^sub>i\<^sub>2 \<sim> lo : sz\<^sub>l\<^sub>o\<^sub>2)\<close>
-  unfolding xtract.simps by (rule step_exps_concatI)
-
-lemma concat_bit_take_bit_drop_bit: \<open>concat_bit n (take_bit n x) (take_bit m (drop_bit n x)) = take_bit (m + n) x\<close>
-  unfolding concat_bit_eq 
-  unfolding take_bit_take_bit min.idem
-  unfolding push_bit_take_bit add.commute[of \<open>take_bit n _\<close>]
-  apply (subst take_bit_plus_push_bit_drop_bit[of m n \<open>x\<close>])
-  unfolding add.commute[of m] ..
-
-lemma nat_concat_bit_take_bit_drop_bit: \<open>nat (concat_bit n (int (take_bit n x)) (int (take_bit m (drop_bit n x)))) = take_bit (m + n) x\<close>
-  unfolding concat_bit_eq take_bit_of_nat push_bit_of_nat nat_int_add concat_bit_take_bit_drop_bit 
-            take_bit_take_bit min.idem push_bit_take_bit add.commute[of \<open>take_bit n _\<close>]
-  apply (subst take_bit_plus_push_bit_drop_bit[of m n \<open>x\<close>])
-  unfolding add.commute[of m] ..
-
-lemma concat_2_bytes: \<open>\<lbrakk>0 < n; 0 < m\<rbrakk> \<Longrightarrow> ((ext num\<^sub>v \<Colon> sz \<sim> hi : (sz\<^sub>l\<^sub>o\<^sub>1 + m + n - 1) \<sim> lo : (sz\<^sub>l\<^sub>o\<^sub>1 + n)) \<cdot> ext num\<^sub>v \<Colon> sz \<sim> hi : (sz\<^sub>l\<^sub>o\<^sub>1 + n - 1) \<sim> lo : sz\<^sub>l\<^sub>o\<^sub>1) = ext num\<^sub>v \<Colon> sz \<sim> hi : (sz\<^sub>l\<^sub>o\<^sub>1 + m + n - 1) \<sim> lo : sz\<^sub>l\<^sub>o\<^sub>1\<close>
-  unfolding bv_concat.simps xtract.simps apply simp
-  unfolding nat_concat_bit_take_bit_drop_bit[symmetric] drop_bit_drop_bit add.commute[of n]
-  ..
-
-lemma concat_2_8bytes: \<open>((ext num\<^sub>v \<Colon> sz \<sim> hi : (sz\<^sub>l\<^sub>o\<^sub>1 + 15) \<sim> lo : (sz\<^sub>l\<^sub>o\<^sub>1 + 8)) \<cdot> ext num\<^sub>v \<Colon> sz \<sim> hi : (sz\<^sub>l\<^sub>o\<^sub>1 + 7) \<sim> lo : sz\<^sub>l\<^sub>o\<^sub>1) = ext num\<^sub>v \<Colon> sz \<sim> hi : (sz\<^sub>l\<^sub>o\<^sub>1 + 15) \<sim> lo : sz\<^sub>l\<^sub>o\<^sub>1\<close>
-  using concat_2_bytes[of 8 8 num\<^sub>v sz sz\<^sub>l\<^sub>o\<^sub>1] apply simp
-  unfolding add.commute[of _ sz\<^sub>l\<^sub>o\<^sub>1] by simp
-
-lemma concat_32_16: \<open>((ext num\<^sub>v \<Colon> sz \<sim> hi : 31 \<sim> lo : 24) \<cdot> ext num\<^sub>v \<Colon> sz \<sim> hi : 23 \<sim> lo : 16) = ext num\<^sub>v \<Colon> sz \<sim> hi : 31 \<sim> lo : 16\<close>
-  using concat_2_8bytes[of num\<^sub>v sz 16] by simp
-
-lemma concat_32_8: \<open>((ext num\<^sub>v \<Colon> sz \<sim> hi : 31 \<sim> lo : 16) \<cdot> ext num\<^sub>v \<Colon> sz \<sim> hi : 15 \<sim> lo : 8) = ext num\<^sub>v \<Colon> sz \<sim> hi : 31 \<sim> lo : 8\<close>
-  using concat_2_bytes[of 8 16 num\<^sub>v sz 8] by simp
-
-lemma concat_32_0: \<open>((ext num\<^sub>v \<Colon> sz \<sim> hi : 31 \<sim> lo : 8) \<cdot> ext num\<^sub>v \<Colon> sz \<sim> hi : 7 \<sim> lo : 0) = ext num\<^sub>v \<Colon> sz \<sim> hi : 31 \<sim> lo : 0\<close>
-  using concat_2_bytes[of 8 24 num\<^sub>v sz 0] by simp
-
-(*
-lemma step_exps_concat_32elI:
-  \<open>\<Delta> \<turnstile> ((((ext num\<^sub>v \<Colon> 32 \<sim> hi : 31 \<sim> lo : 24) @ ext num\<^sub>v \<Colon> 32 \<sim> hi : 23 \<sim> lo : 16) @ ext num\<^sub>v \<Colon> 32 \<sim> hi : 15 \<sim> lo : 8) @ ext num\<^sub>v \<Colon> 32 \<sim> hi : 7 \<sim> lo : 0) \<leadsto>* (num\<^sub>v \<Colon> 32)\<close>
-  apply (rule step_exps_concat_lhs.extractI)
-  apply (rule step_concat_lhs.extractI)
-  apply (rule step_concat_extractI)
-  unfolding concat_32_16
-
-  apply (rule step_exps_concat_lhs.extractI)
-  apply (rule step_concat_extractI)
-  unfolding concat_32_8
-
-  unfolding concat_32_0[symmetric]
-*)
-find_theorems Suc "(mod)"
-thm mod_add_right_eq mod_add_left_eq
-
-lemmas Gggggsimps = succ.simps bv_plus.simps mod_add_right_eq mod_add_left_eq xtract.simps drop_bit_0 mod_Suc_eq Suc3_eq_add_3
-
-thm step_load_addrI step_load_memI.syntaxs
-thm step_load_byte_from_nextI.syntaxs
-thm step_load_byteI
-thm step_load_byteI.syntaxs
-thm step_load_word_elI
-lemmas nat_concat_bit_take_bit_drop_bit2 = 
-  nat_concat_bit_take_bit_drop_bit[of _ \<open>drop_bit _ _\<close> _, unfolded drop_bit_drop_bit]
-
 lemma xtract_concat_consecutive:
   assumes \<open>x2 > x3\<close> \<open>x3 > x4\<close>
     shows \<open>(ext num \<Colon> x1 \<sim> hi : x2 \<sim> lo : x3) \<cdot> (ext num \<Colon> x1 \<sim> hi : x3 - 1 \<sim> lo : x4) = (ext num \<Colon> x1 \<sim> hi : x2 \<sim> lo : x4)\<close>
@@ -88,20 +23,20 @@ next
     using assms by fastforce
 qed
 
-lemma xtract64_48_el[simp]: \<open>(ext num \<Colon> 64 \<sim> hi : 63 \<sim> lo : 56) \<cdot> (ext num \<Colon> 64 \<sim> hi : 55 \<sim> lo : 48) = (ext num \<Colon> 64 \<sim> hi : 63 \<sim> lo : 48)\<close>
-  by (rule xtract_concat_consecutive[of 56 63 48, simplified])
-lemma xtract64_40_el[simp]: \<open>(ext num \<Colon> 64 \<sim> hi : 63 \<sim> lo : 48) \<cdot> (ext num \<Colon> 64 \<sim> hi : 47 \<sim> lo : 40) = (ext num \<Colon> 64 \<sim> hi : 63 \<sim> lo : 40)\<close>
-  by (rule xtract_concat_consecutive[of 48 63 40, simplified])
-lemma xtract64_32_el[simp]: \<open>(ext num \<Colon> 64 \<sim> hi : 63 \<sim> lo : 40) \<cdot> (ext num \<Colon> 64 \<sim> hi : 39 \<sim> lo : 32) = (ext num \<Colon> 64 \<sim> hi : 63 \<sim> lo : 32)\<close>
-  by (rule xtract_concat_consecutive[of 40 63 32, simplified])
-lemma xtract64_24_el[simp]: \<open>(ext num \<Colon> 64 \<sim> hi : 63 \<sim> lo : 32) \<cdot> (ext num \<Colon> 64 \<sim> hi : 31 \<sim> lo : 24) = (ext num \<Colon> 64 \<sim> hi : 63 \<sim> lo : 24)\<close>
-  by (rule xtract_concat_consecutive[of 32 63 24, simplified])
-lemma xtract64_16_el[simp]: \<open>(ext num \<Colon> 64 \<sim> hi : 63 \<sim> lo : 24) \<cdot> (ext num \<Colon> 64 \<sim> hi : 23 \<sim> lo : 16) = (ext num \<Colon> 64 \<sim> hi : 63 \<sim> lo : 16)\<close>
-  by (rule xtract_concat_consecutive[of 24 63 16, simplified])
-lemma xtract64_8_el[simp]:  \<open>(ext num \<Colon> 64 \<sim> hi : 63 \<sim> lo : 16) \<cdot> (ext num \<Colon> 64 \<sim> hi : 15 \<sim> lo :  8) = (ext num \<Colon> 64 \<sim> hi : 63 \<sim> lo :  8)\<close>
-  by (rule xtract_concat_consecutive[of 16 63 8, simplified])
-lemma xtract64_0_el[simp]:  \<open>(ext num \<Colon> 64 \<sim> hi : 63 \<sim> lo : 8) \<cdot> (ext num \<Colon> 64 \<sim> hi : 7 \<sim> lo :  0) = (ext num \<Colon> 64 \<sim> hi : 63 \<sim> lo :  0)\<close>
-  by (rule xtract_concat_consecutive[of 8 63 0, simplified])
+lemmas xtract64_48_el[simp] = xtract_concat_consecutive[of 56 63 48, simplified]
+lemmas xtract64_40_el[simp] = xtract_concat_consecutive[of 48 63 40, simplified]
+lemmas xtract64_32_el[simp] = xtract_concat_consecutive[of 40 63 32, simplified]
+lemmas xtract64_24_el[simp] = xtract_concat_consecutive[of 32 63 24, simplified]
+lemmas xtract64_16_el[simp] = xtract_concat_consecutive[of 24 63 16, simplified]
+lemmas xtract64_8_el[simp]  = xtract_concat_consecutive[of 16 63 8, simplified]
+lemmas xtract64_0_el[simp]  = xtract_concat_consecutive[of 8 63 0, simplified]
+lemmas xtract64_15_0[simp]  = xtract_concat_consecutive[of 8 15 0, simplified]
+lemmas xtract64_23_0[simp]  = xtract_concat_consecutive[of 16 23 0, simplified]
+lemmas xtract64_31_0[simp]  = xtract_concat_consecutive[of 24 31 0, simplified]
+lemmas xtract64_39_0[simp]  = xtract_concat_consecutive[of 32 39 0, simplified]
+lemmas xtract64_47_0[simp]  = xtract_concat_consecutive[of 40 47 0, simplified]
+lemmas xtract64_55_0[simp]  = xtract_concat_consecutive[of 48 55 0, simplified]
+lemmas xtract64_63_0[simp]  = xtract_concat_consecutive[of 56 63 0, simplified]
 
 lemmas xtract64_els = xtract64_48_el xtract64_40_el xtract64_32_el xtract64_24_el xtract64_16_el
                       xtract64_8_el  xtract64_0_el
@@ -111,48 +46,87 @@ lemma step_exps_concat_word64_elI: \<open>\<Delta> \<turnstile> ((((((((
   ext num \<Colon> 64 \<sim> hi : 47 \<sim> lo : 40) @ ext num \<Colon> 64 \<sim> hi : 39 \<sim> lo : 32) @
   ext num \<Colon> 64 \<sim> hi : 31 \<sim> lo : 24) @ ext num \<Colon> 64 \<sim> hi : 23 \<sim> lo : 16) @
   ext num \<Colon> 64 \<sim> hi : 15 \<sim> lo :  8) @ ext num \<Colon> 64 \<sim> hi :  7 \<sim> lo :  0) \<leadsto>* (ext num \<Colon> 64 \<sim> hi : 63 \<sim> lo : 0)\<close>  
-  apply solve_expsI
-  unfolding xtract64_els
-  apply solve_expsI
-  unfolding xtract64_els
-  apply solve_expsI
-  unfolding xtract64_els
-  apply solve_expsI
-  unfolding xtract64_els
-  apply solve_expsI
-  unfolding xtract64_els
-  apply solve_expsI
-  unfolding xtract64_els
-  unfolding xtract64_0_el[symmetric]
-  by (rule step_exps_concatI.xtract.xtract)
+  apply (solve_expsI simp: xtract64_els)
+  by (unfold xtract64_els, unfold xtract64_0_el[symmetric], rule step_exps_concatI.xtract.xtract)
 
-lemma step_exps_load_word64_elI: \<open>\<Delta> \<turnstile> (storage64 v num\<^sub>a 64 num\<^sub>v)[num\<^sub>a \<Colon> 64, el]:u64 \<leadsto>* (ext num\<^sub>v \<Colon> 64 \<sim> hi : 63 \<sim> lo : 0)\<close>
-  apply solve_expsI
+lemma step_exps_load_word64_elI: \<open>\<Delta> \<turnstile> (storage_el64 v (num\<^sub>a \<Colon> 64) (num\<^sub>v \<Colon> 64))[num\<^sub>a \<Colon> 64, el]:u64 \<leadsto>* (ext num\<^sub>v \<Colon> 64 \<sim> hi : 63 \<sim> lo : 0)\<close>
+  apply (solve_exps_intI \<open>rule step_exps_concat_word64_elI\<close>)
   apply simp
-  apply solve_expsI
-  sorry
+  by (solve_exps_intI \<open>rule step_exps_concat_word64_elI\<close>)
 
-lemma step_exps_store_word64_elI: 
-  assumes \<open>type mem = mem\<langle>64, 8\<rangle>\<close>
-    shows \<open>\<Delta> \<turnstile> (Val mem) with [num\<^sub>a \<Colon> 64, el]:u64 \<leftarrow> (num\<^sub>v \<Colon> 64) \<leadsto>* (storage64 v num\<^sub>a 64 num\<^sub>v)\<close>
+lemma step_exps_load_word64_beI: \<open>\<Delta> \<turnstile> (storage_be64 v (num\<^sub>a \<Colon> 64) (num\<^sub>v \<Colon> 64))[num\<^sub>a \<Colon> 64, be]:u64 \<leadsto>* (ext num\<^sub>v \<Colon> 64 \<sim> hi : 63 \<sim> lo : 0)\<close>
+  apply (solve_expsI, simp)+
+  unfolding xtract64_63_0[symmetric] by solve_expsI
+
+lemma nested_extract_within': 
+  assumes  \<open>sz\<^sub>l\<^sub>o' \<le> sz\<^sub>h\<^sub>i'\<close> and \<open>sz\<^sub>h\<^sub>i' + sz\<^sub>l\<^sub>o \<le> sz\<^sub>h\<^sub>i\<close>
+    shows \<open>(ext (ext num \<Colon> sz \<sim> hi : sz\<^sub>h\<^sub>i \<sim> lo : sz\<^sub>l\<^sub>o) \<sim> hi : sz\<^sub>h\<^sub>i' \<sim> lo : sz\<^sub>l\<^sub>o') = (ext num \<Colon> sz \<sim> hi : (sz\<^sub>h\<^sub>i' + sz\<^sub>l\<^sub>o) \<sim> lo : (sz\<^sub>l\<^sub>o' + sz\<^sub>l\<^sub>o))\<close>
+  using assms unfolding xtract.simps take_bit_drop_bit by auto
+
+lemma nested_extract_within: 
+  assumes \<open>sz\<^sub>l\<^sub>o' + sz\<^sub>l\<^sub>o \<le> sz\<^sub>h\<^sub>i\<close>
+    shows \<open>(ext (ext num \<Colon> sz \<sim> hi : sz\<^sub>h\<^sub>i \<sim> lo : sz\<^sub>l\<^sub>o) \<sim> hi : (sz\<^sub>h\<^sub>i - sz\<^sub>l\<^sub>o) \<sim> lo : sz\<^sub>l\<^sub>o') = (ext num \<Colon> sz \<sim> hi : sz\<^sub>h\<^sub>i \<sim> lo : (sz\<^sub>l\<^sub>o' + sz\<^sub>l\<^sub>o))\<close>
+  using assms using nested_extract_within'[where sz\<^sub>h\<^sub>i'= \<open>sz\<^sub>h\<^sub>i - sz\<^sub>l\<^sub>o\<close> and sz\<^sub>l\<^sub>o = sz\<^sub>l\<^sub>o and sz\<^sub>l\<^sub>o' = sz\<^sub>l\<^sub>o' and sz\<^sub>h\<^sub>i = sz\<^sub>h\<^sub>i and num = num and sz = sz]
+  apply auto
+  using add_le_imp_le_diff by blast
+
+
+
+lemmas xtract_nested_63_8_55_8[simp]  = nested_extract_within [of  8  8 63, simplified]
+lemmas xtract_nested_63_16_47_8[simp] = nested_extract_within [of  8 16 63, simplified]
+lemmas xtract_nested_63_24_39_8[simp] = nested_extract_within [of  8 24 63, simplified]
+lemmas xtract_nested_63_32_31_8[simp] = nested_extract_within [of  8 32 63, simplified]
+lemmas xtract_nested_63_40_23_8[simp] = nested_extract_within [of  8 40 63, simplified]
+lemmas xtract_nested_63_48_15_8[simp] = nested_extract_within [of  8 48 63, simplified]
+lemmas xtract_nested_55_0_47_0[simp]  = nested_extract_within'[of  0 47  0 55, simplified]
+lemmas xtract_nested_47_0_39_0[simp]  = nested_extract_within'[of  0 39  0 47, simplified]
+lemmas xtract_nested_39_0_31_0[simp]  = nested_extract_within'[of  0 31  0 39, simplified]
+lemmas xtract_nested_31_0_23_0[simp]  = nested_extract_within'[of  0 23  0 31, simplified]
+lemmas xtract_nested_23_0_15_0[simp]  = nested_extract_within'[of  0 15  0 23, simplified]
+lemmas xtract_nested_15_0_7_0[simp]   = nested_extract_within'[of  0  7  0 15, simplified]
+lemmas xtract_nested_63_8_7_0[simp]   = nested_extract_within'[of  0  7  8 63,  simplified]
+lemmas xtract_nested_63_16_7_0[simp]  = nested_extract_within'[of  0  7 16 63, simplified]
+lemmas xtract_nested_63_24_7_0[simp]  = nested_extract_within'[of  0  7 24 63, simplified]
+lemmas xtract_nested_63_32_7_0[simp]  = nested_extract_within'[of  0  7 32 63, simplified]
+lemmas xtract_nested_63_40_7_0[simp]  = nested_extract_within'[of  0  7 40 63, simplified]
+lemmas xtract_nested_63_48_7_0[simp]  = nested_extract_within'[of  0  7 48 63, simplified]
+lemmas xtract_nested_55_0_55_48[simp] = nested_extract_within'[of 48 55  0 55, simplified]
+lemmas xtract_nested_47_0_47_40[simp] = nested_extract_within'[of 40 47  0 47, simplified]
+lemmas xtract_nested_39_0_39_32[simp] = nested_extract_within'[of 32 39  0 39, simplified]
+lemmas xtract_nested_31_0_31_24[simp] = nested_extract_within'[of 24 31  0 31, simplified]
+lemmas xtract_nested_23_0_23_16[simp] = nested_extract_within'[of 16 23  0 23, simplified]
+lemmas xtract_nested_15_0_15_8[simp]  = nested_extract_within'[of  8 15  0 15, simplified]
+
+lemma step_exps_store_word64_elI:
+  assumes \<open>type mem = mem\<langle>sz\<^sub>a\<^sub>d\<^sub>d\<^sub>r, 8\<rangle>\<close>
+    shows \<open>\<Delta> \<turnstile> (Val mem) with [num\<^sub>a\<^sub>d\<^sub>d\<^sub>r \<Colon> sz\<^sub>a\<^sub>d\<^sub>d\<^sub>r, el]:u64 \<leftarrow> (num\<^sub>v \<Colon> 64) \<leadsto>* (storage_el64 mem (num\<^sub>a\<^sub>d\<^sub>d\<^sub>r \<Colon> sz\<^sub>a\<^sub>d\<^sub>d\<^sub>r) (num\<^sub>v \<Colon> 64))\<close>
   using assms apply -
-  apply solve_expsI
-  using step_exps_store_word_elI.storage.word
-  apply solve_expsI
-  apply simp
-  apply solve_expsI
-  sorry
+  apply (solve_expsI, simp)+
+  by solve_expsI
 
-lemma word8_refl_load_rev_ext_concat_word32: 
-  assumes \<open>num < 2 ^ 32\<close>
-    shows \<open>\<Delta> \<turnstile> v[num\<^sub>a \<Colon> 64 \<leftarrow> ext num \<Colon> 32 \<sim> hi : 7 \<sim> lo : 0, 8][succ (num\<^sub>a \<Colon> 64) \<leftarrow> ext num \<Colon> 32 \<sim> hi : 15 \<sim> lo : 8, 8][succ (succ (num\<^sub>a \<Colon> 64)) \<leftarrow> ext num \<Colon> 32 \<sim> hi : 23 \<sim> lo : 16, 8][succ (succ (succ (num\<^sub>a \<Colon> 64))) \<leftarrow> ext num \<Colon> 32 \<sim> hi : 31 \<sim> lo : 24, 8][num\<^sub>a \<Colon> 64, el]:u32 \<leadsto>* (num \<Colon> 32)\<close>
-  apply (subgoal_tac \<open>\<Delta> \<turnstile> v[num\<^sub>a \<Colon> 64 \<leftarrow> ext num \<Colon> 32 \<sim> hi : 7 \<sim> lo : 0, 8][succ (num\<^sub>a \<Colon> 64) \<leftarrow> ext num \<Colon> 32 \<sim> hi : 15 \<sim> lo : 8, 8][succ (succ (num\<^sub>a \<Colon> 64)) \<leftarrow> ext num \<Colon> 32 \<sim> hi : 23 \<sim> lo : 16, 8][succ (succ (succ (num\<^sub>a \<Colon> 64))) \<leftarrow> ext num \<Colon> 32 \<sim> hi : 31 \<sim> lo : 24, 8][num\<^sub>a \<Colon> 64, el]:u32 \<leadsto>* ((((ext num \<Colon> 32 \<sim> hi : 31 \<sim> lo : 24) \<cdot>
-      ext num \<Colon> 32 \<sim> hi : 23 \<sim> lo : 16) \<cdot>
-     ext num \<Colon> 32 \<sim> hi : 15 \<sim> lo : 8) \<cdot>
-    ext num \<Colon> 32 \<sim> hi : 7 \<sim> lo : 0)\<close>)
-  apply (metis assms extract_concat32)
-  unfolding xtract.simps apply (simp add: bv_plus.simps del: bv_concat.simps)
-  using word8_refl_load_rev_word32I by blast
+interpretation step_exps_store_word64_elI: store_gt8_syntax \<open>\<lambda>e\<^sub>1 v\<^sub>1 e\<^sub>2 w\<^sub>2 sz\<^sub>2 e\<^sub>3 v\<^sub>3. (\<And>\<Delta>. \<Delta> \<turnstile> e\<^sub>1 with [e\<^sub>2, el]:u64 \<leftarrow> e\<^sub>3 \<leadsto>* (storage_el64 v\<^sub>1 w\<^sub>2 v\<^sub>3))\<close> 64
+  by (standard, rule step_exps_store_word64_elI)
 
+lemma step_exps_store_word64_beI: 
+  assumes \<open>type mem = mem\<langle>sz\<^sub>a\<^sub>d\<^sub>d\<^sub>r, 8\<rangle>\<close>
+    shows \<open>\<Delta> \<turnstile> (Val mem) with [num\<^sub>a\<^sub>d\<^sub>d\<^sub>r \<Colon> sz\<^sub>a\<^sub>d\<^sub>d\<^sub>r, be]:u64 \<leftarrow> (num\<^sub>v \<Colon> 64) \<leadsto>* (storage_be64 mem (num\<^sub>a\<^sub>d\<^sub>d\<^sub>r \<Colon> sz\<^sub>a\<^sub>d\<^sub>d\<^sub>r) (num\<^sub>v \<Colon> 64))\<close>
+  using assms apply -
+  apply (solve_expsI, simp)+
+  by solve_expsI
+
+interpretation step_exps_store_word64_beI: store_gt8_syntax \<open>\<lambda>e\<^sub>1 v\<^sub>1 e\<^sub>2 w\<^sub>2 sz\<^sub>2 e\<^sub>3 v\<^sub>3. (\<And>\<Delta>. \<Delta> \<turnstile> e\<^sub>1 with [e\<^sub>2, be]:u64 \<leftarrow> e\<^sub>3 \<leadsto>* (storage_be64 v\<^sub>1 w\<^sub>2 v\<^sub>3))\<close> 64
+  by (standard, rule step_exps_store_word64_beI)
+
+text \<open>The 64bit solver\<close>
+
+method solve_exps_64I = (
+  rule step_exps_concat_word64_elI |
+
+  (rule step_exps_store_word64_elI, solve_typeI) |
+  (rule step_exps_store_word64_beI, solve_typeI) |
+
+  (rule step_exps_load_word64_elI) |
+  (rule step_exps_load_word64_beI)
+)
 
 end
